Matroid/ForMathlib/Relation.lean
@@ -1,11 +1,15 @@
-import Mathlib.Data.Setoid.Basic
+import Mathlib.Data.Set.Pairwise.Basic
 import Mathlib.Order.Closure
 
 open Set Function
-namespace Relation
 
-variable {α β γ ι : Type*} {a b c : α} {x y z : β} {u v w : γ} {f : ι → α}
+variable {α β γ ι : Type*} {a b c : α} {x y z : β} {u v w : γ} {f : β → α}
   {r r' : α → β → Prop} {s s' : β → γ → Prop} {t t' : α → γ → Prop}
+
+lemma trans' [Trans r s t] (hr : r a x) (hs : s x u) : t a u :=
+  Trans.trans hr hs
+
+namespace Relation
 
 /--
 # Relation
@@ -15,11 +19,10 @@ variable {α β γ ι : Type*} {a b c : α} {x y z : β} {u v w : γ} {f : ι �
 converse is `flip`
 -/
 
+scoped macro:1050 r:term "ᵀ" : term => `(flip $r)
+
 @[simp]
 lemma compl_apply : (r a x)ᶜ ↔ ¬r a x := Iff.rfl
-
-lemma trans' [Trans r s t] (hr : r a x) (hs : s x u) : t a u :=
-  Trans.trans hr hs
 
 def domain (r : α → β → Prop) : Set α := {x | ∃ y, r x y}
 
@@ -36,10 +39,10 @@ lemma left_mem_domain (hr : r a x) : a ∈ domain r := ⟨x, hr⟩
 lemma right_mem_codomain (hr : r a x) : x ∈ codomain r := ⟨a, hr⟩
 
 @[simp]
-lemma domain_flip (r : α → β → Prop) : domain (flip r) = codomain r := rfl
+lemma domain_flip (r : α → β → Prop) : domain rᵀ = codomain r := rfl
 
 @[simp]
-lemma codomain_flip (r : α → β → Prop) : codomain (flip r) = domain r := rfl
+lemma codomain_flip (r : α → β → Prop) : codomain rᵀ = domain r := rfl
 
 lemma domain_comp (r : α → β → Prop) (s : β → γ → Prop) : domain (Comp r s) ⊆ domain r := by
   rintro x ⟨c, b, hrxb, hsbc⟩
@@ -57,6 +60,57 @@ lemma codomain_mono (h : r ≤ r') : codomain r ⊆ codomain r' := by
   rintro y ⟨x, hry⟩
   exact ⟨x, h _ _ hry⟩
 
+/-- Double composition of `r` of the converse of `s`-/
+def Domp (r s : α → β → Prop) : α → β → Prop := Comp (Comp r sᵀ) r
+
+lemma domp_def (r s : α → β → Prop) : Domp r s = Comp (Comp r sᵀ) r := rfl
+
+lemma domp_def' (r s : α → β → Prop) : Domp r s = Comp r (Comp sᵀ r) := by
+  rw [← comp_assoc]
+  rfl
+
+lemma domain_domp (r s : α → β → Prop) : domain (Domp r s) ⊆ domain r := by
+  rw [domp_def']
+  exact domain_comp r (Comp (flip s) r)
+
+lemma codomain_domp (r s : α → β → Prop) : codomain (Domp r s) ⊆ codomain r := by
+  rw [domp_def]
+  exact codomain_comp (Comp r sᵀ) r
+
+lemma le_domp_self (r : α → β → Prop) : r ≤ Domp r r :=
+  fun a b hrab => ⟨a, ⟨b, hrab, hrab⟩, hrab⟩
+
+class Domple (r : α → β → Prop) : Prop where
+  domple : Domp r r ≤ r
+
+lemma domp_le (r : α → β → Prop) [Domple r] : Domp r r ≤ r := Domple.domple
+
+@[simp]
+lemma domp_eq (r : α → β → Prop) [Domple r] : Domp r r = r :=
+  antisymm (domp_le r) (le_domp_self r)
+
+instance [Domple r] : Trans r (Comp rᵀ r) r where
+  trans := by
+    rintro a x y hrax ⟨b, hrbx, hrby⟩
+    exact domp_le r a y ⟨b, ⟨x, hrax, hrbx⟩, hrby⟩
+
+instance [Domple r] : Trans (Comp r rᵀ) r r where
+  trans := by
+    rintro a b x ⟨y, hray, hrby⟩ hrbx
+    exact domp_le r a x ⟨b, ⟨y, hray, hrby⟩, hrbx⟩
+
+lemma domple_left [Domple r] (hrax : r a x) (hrbx : r b x) (hray : r a y) : r b y :=
+  domp_le r b y ⟨a, ⟨x, hrbx, hrax⟩, hray⟩
+
+lemma domple_left_iff [Domple r] (hrax : r a x) (hrbx : r b x) : r a y ↔ r b y :=
+  ⟨domple_left hrax hrbx, domple_left hrbx hrax⟩
+
+lemma domple_right [Domple r] (hrax : r a x) (hray : r a y) (hrbx : r b x) : r b y :=
+  domp_le r b y ⟨a, ⟨x, hrbx, hrax⟩, hray⟩
+
+lemma domple_right_iff [Domple r] (hrax : r a x) (hray : r a y) : r b x ↔ r b y :=
+  ⟨domple_right hrax hray, domple_right hray hrax⟩
+
 
 def fiber (r : α → β → Prop) (x : β) : Set α := {a | r a x}
 
@@ -67,15 +121,30 @@ lemma mem_fiber_iff (r : α → β → Prop) : a ∈ fiber r x ↔ r a x := Iff.
 lemma fiber_empty : fiber r x = ∅ ↔ x ∉ codomain r := by
   simp [fiber, eq_empty_iff_forall_notMem]
 
+lemma fiber_eq_or_disjoint [Domple r] :
+    fiber r x = fiber r y ∨ Disjoint (fiber r x) (fiber r y) := by
+  rw [or_iff_not_imp_right, not_disjoint_iff_nonempty_inter]
+  rintro ⟨a, hax, hay⟩
+  ext b
+  simp only [mem_fiber_iff] at hax hay ⊢
+  exact domple_right_iff hax hay
+
+lemma fiber_eq_of_mem [Domple r] (hrax : r a x) (hray : r a y) : fiber r x = fiber r y := by
+  apply fiber_eq_or_disjoint.resolve_right
+  rw [not_disjoint_iff_nonempty_inter]
+  use a
+  exact ⟨hrax, hray⟩
+
+
 def image (r : α → β → Prop) (S : Set α) : Set β := {x | ∃ a ∈ S, r a x}
 
 def preimage (r : α → β → Prop) (S : Set β) : Set α := {a | ∃ x ∈ S, r a x}
 
 @[simp]
-lemma image_flip (r : α → β → Prop) (S : Set β) : image (flip r) S = preimage r S := rfl
+lemma image_flip (r : α → β → Prop) (S : Set β) : image rᵀ S = preimage r S := rfl
 
 @[simp]
-lemma preimage_flip (r : α → β → Prop) (S : Set α) : preimage (flip r) S = image r S := rfl
+lemma preimage_flip (r : α → β → Prop) (S : Set α) : preimage rᵀ S = image r S := rfl
 
 @[simp]
 lemma mem_image_iff (r : α → β → Prop) (S : Set α) :
@@ -90,7 +159,17 @@ lemma sUnion_fiber (r : α → β → Prop) (S : Set β) : ⋃₀ (fiber r '' S)
   ext a
   simp
 
+@[simp]
+lemma image_domain (r : α → β → Prop) : image r (domain r) = codomain r := by
+  ext x
+  simp only [mem_image_iff, mem_domain_iff, mem_codomain_iff]
+  exact ⟨fun ⟨a, _, hrax⟩ => ⟨a, hrax⟩, fun ⟨a, hrax⟩ => ⟨a, ⟨x, hrax⟩, hrax⟩⟩
 
+@[simp]
+lemma preimage_codomain (r : α → β → Prop) : preimage r (codomain r) = domain r := by
+  ext a
+  simp only [mem_preimage_iff, mem_codomain_iff, mem_domain_iff]
+  exact ⟨fun ⟨x, _, hrax⟩ => ⟨x, hrax⟩, fun ⟨x, hrax⟩ => ⟨x, ⟨a, hrax⟩, hrax⟩⟩
 
 
 
@@ -111,6 +190,12 @@ class IsRightTotal (r : α → β → Prop) : Prop where
 
 lemma right_total (r : α → β → Prop) [IsRightTotal r] : ∀ x, ∃ a, r a x :=
   IsRightTotal.is_right_total
+
+@[simp]
+lemma codomain_univ (r : α → β → Prop) [IsRightTotal r] : codomain r = univ := by
+  ext y
+  simp only [mem_codomain_iff, mem_univ, iff_true]
+  exact right_total r y
 
 class IsTotal (r : α → β → Prop) : Prop extends IsLeftTotal r, IsRightTotal r
 
@@ -142,22 +227,42 @@ lemma mem_fibers_iff (r : α → β → Prop) (S : Set α) :
     S ∈ fibers r ↔ ∃ x ∈ codomain r, fiber r x = S := by
   simp [fibers]
 
-lemma fibers_sSup_univ [IsLeftTotal r] : ⋃₀ fibers r = univ := by
-  ext a
-  simp only [fibers, fiber, mem_sUnion, mem_image, mem_codomain_iff, exists_exists_and_eq_and,
-    mem_setOf_eq, mem_univ, iff_true]
-  obtain ⟨x, hrax⟩ := left_total r a
-  exact ⟨x, ⟨a, hrax⟩, hrax⟩
+lemma emptySet_notMem_fibers (r : α → β → Prop) : ∅ ∉ fibers r := by
+  rintro ⟨x, ⟨a, hrax⟩, heq⟩
+  have : a ∈ fiber r x := hrax
+  simp only [mem_empty_iff_false, heq] at this
 
-lemma fibers_pairwiseDisjoint [IsLeftUnique r] :
-    ∀ S T, S ∈ fibers r → T ∈ fibers r → S ≠ T → Disjoint S T := by
-  rintro S T ⟨b, -, rfl⟩ ⟨b', -, rfl⟩ hST
+lemma nonempty_of_mem_fibers {S : Set α} (hS : S ∈ fibers r) : S.Nonempty := by
+  obtain ⟨x, ⟨a, hax⟩, rfl⟩ := hS
+  exact ⟨a, hax⟩
+
+@[simp]
+lemma sUnion_fibers (r : α → β → Prop) : ⋃₀ fibers r = domain r := by
+  simp [fibers]
+
+lemma fibers_pairwiseDisjoint' [IsLeftUnique r] : (fibers r).PairwiseDisjoint id := by
+  rintro S ⟨b, -, rfl⟩ T ⟨b', -, rfl⟩ hST
+  change Disjoint (fiber r b) (fiber r b')
   rw [disjoint_iff_inter_eq_empty]
   ext a
   simp only [mem_inter_iff, mem_fiber_iff, mem_empty_iff_false, iff_false, not_and]
   rintro hrxb hrxb'
   obtain rfl := left_unique r a b b' hrxb hrxb'
   exact hST rfl
+
+lemma fibers_pairwiseDisjoint [Domple r] :
+    (fibers r).PairwiseDisjoint id := by
+  rintro S ⟨x, ⟨a, hrax⟩, rfl⟩ T ⟨y, ⟨b, hrby⟩, rfl⟩ hST
+  change Disjoint (fiber r x) (fiber r y)
+  rw [disjoint_iff_inter_eq_empty]
+  ext b
+  simp only [mem_inter_iff, mem_fiber_iff, mem_empty_iff_false, iff_false, not_and]
+  rintro hrbx hrby
+  refine hST ?_
+  ext c
+  simp only [mem_fiber_iff]
+  exact domple_right_iff hrbx hrby
+
 
 
 instance : HasSubset (α → β → Prop) where
@@ -184,13 +289,13 @@ def rightRestrict (r : α → β → Prop) (S : Set β) : α → β → Prop :=
 
 notation r " |ᵣ " S => rightRestrict r S
 
-def leftResidual (r : α → β → Prop) (s : α → γ → Prop) : β → γ → Prop :=
-  (Comp (flip r) sᶜ)ᶜ
-notation r " \\ " s => leftResidual r s
+-- def leftResidual (r : α → β → Prop) (s : α → γ → Prop) : β → γ → Prop :=
+--   (Comp rᵀ sᶜ)ᶜ
+-- notation r " \\ " s => leftResidual r s
 
-def rightResidual (r : α → β → Prop) (s : γ → β → Prop) : α → γ → Prop :=
-  (Comp rᶜ (flip s))ᶜ
-notation r " / " s => rightResidual r s
+-- def rightResidual (r : α → β → Prop) (s : γ → β → Prop) : α → γ → Prop :=
+--   (Comp rᶜ sᵀ)ᶜ
+-- notation r " / " s => rightResidual r s
 
 
 
@@ -223,7 +328,7 @@ lemma comp_le (r : α → β → Prop) (s : β → γ → Prop) (t : α → γ �
 --   simp only [rightResidual, Pi.compl_apply, compl_iff_not, not_not]
 --   use c, this, hsbc
 
--- lemma le_rightResidual {r : α → β → Prop} {s : β → γ → Prop} {t : α → γ → Prop} [Schroder r s t] :
+-- lemma le_rightResidual {r : α → β → Prop} {s : β → γ → Prop} {t : α → γ → Prop} [Schroder r s t]:
 --     r ≤ t / s := by
 --   rw [← Schroder_rightResidual]
 --   exact comp_le
@@ -293,8 +398,14 @@ instance : IsSymm α ⊥ where
 instance : IsTrans α ⊥ where
   trans := by simp
 
-instance [IsRefl α r] : IsRefl ι (r on f) where
-  refl i := refl (f i)
+instance [IsRefl α r] : IsRefl β (r on f) where
+  refl a := refl (f a)
+
+instance [IsSymm α r] : IsSymm β (r on f) where
+  symm a _ := symm (a := f a)
+
+instance [IsTrans α r] : IsTrans β (r on f) where
+  trans a _ _ := trans' (a := f a)
 
 instance [IsSymm α r] [IsSymm α s] : IsSymm α (r ⊔ s) := by
   refine ⟨fun a b h ↦ ?_⟩
@@ -303,28 +414,29 @@ instance [IsSymm α r] [IsSymm α s] : IsSymm α (r ⊔ s) := by
 instance [IsSymm α r] [IsSymm α s] : IsSymm α (r ⊓ s) :=
   ⟨fun a b ⟨hr, hs⟩ ↦ by simp [symm hr, symm hs]⟩
 
-instance [IsSymm α r] : IsSymm α (flip r) where
+instance [IsSymm α r] : IsSymm α rᵀ where
   symm _ _ := symm_of r
 
-lemma sSup_symm {s : Set (α → α → Prop)} (hs : ∀ r ∈ s, IsSymm α r) : IsSymm α (sSup s) where
-  symm a b h := by
-    induction h with
-    | intro w h =>
-      simp only [mem_range, eq_iff_iff, Subtype.exists, exists_prop, exists_exists_and_eq_and,
-        binary_relation_sSup_iff s] at h ⊢
-      obtain ⟨⟨r, hrs, hrw⟩, hw⟩ := h
-      have := hs r hrs
-      exact ⟨r, hrs, symm <| hrw.mpr hw⟩
+lemma sSup_symmtric {s : Set (α → α → Prop)} (hs : ∀ r ∈ s, IsSymm α r) : Symmetric (sSup s) := by
+  rintro a b h
+  induction h with
+  | intro w h =>
+    simp only [mem_range, eq_iff_iff, Subtype.exists, exists_prop, exists_exists_and_eq_and,
+      binary_relation_sSup_iff s] at h ⊢
+    obtain ⟨⟨r, hrs, hrw⟩, hw⟩ := h
+    have := hs r hrs
+    exact ⟨r, hrs, symm <| hrw.mpr hw⟩
 
-lemma sInf_symm {s : Set (α → α → Prop)} (hs : ∀ r ∈ s, IsSymm α r) : IsSymm α (sInf s) where
-  symm a b := by
-    simp_rw [binary_relation_sInf_iff s]
-    exact fun h r hrs => let := hs r hrs; symm (h r hrs)
+lemma sInf_symmtric {s : Set (α → α → Prop)} (hs : ∀ r ∈ s, IsSymm α r) : Symmetric (sInf s) := by
+  rintro a b
+  simp_rw [binary_relation_sInf_iff s]
+  exact fun h r hrs => let := hs r hrs; symm (h r hrs)
 
-lemma sInf_trans {s : Set (α → α → Prop)} (hs : ∀ r ∈ s, IsTrans α r) : IsTrans α (sInf s) where
-  trans a b c := by
-    simp_rw [binary_relation_sInf_iff s]
-    exact fun hab hbc r hrs => let := hs r hrs; trans_of _ (hab r hrs) (hbc r hrs)
+lemma sInf_transitive {s : Set (α → α → Prop)} (hs : ∀ r ∈ s, IsTrans α r) :
+    Transitive (sInf s) := by
+  rintro a b c
+  simp_rw [binary_relation_sInf_iff s]
+  exact fun hab hbc r hrs => let := hs r hrs; trans' (hab r hrs) (hbc r hrs)
 
 lemma domain_eq_codomain (r : α → α → Prop) [IsSymm α r] : domain r = codomain r := by
   ext a
@@ -334,7 +446,7 @@ lemma domain_eq_codomain (r : α → α → Prop) [IsSymm α r] : domain r = cod
 instance [IsTrans α r] [IsTrans α s] : IsTrans α (r ⊓ s) :=
   ⟨fun _ _ _ ⟨hr, hs⟩ ⟨hr', hs'⟩ ↦ ⟨trans_of r hr hr', trans_of s hs hs'⟩⟩
 
-instance [IsTrans α r] : IsTrans α (flip r) where
+instance [IsTrans α r] : IsTrans α rᵀ where
   trans _ _ _ h h' := trans_of r h' h
 
 def TransClosure : ClosureOperator (α → α → Prop) where
@@ -367,13 +479,13 @@ class foo (r : α → α → Prop) where
 
 lemma refl_of_right [foo r] (h : r a b) : r b b := foo.isfoo h
 lemma refl_of_left [foo <| flip r] (h : r a b) : r a a := by
-  change (flip r) a a
+  change rᵀ a a
   exact refl_of_right h
 
 instance [IsSymm α r] [IsTrans α r] : foo r where
   isfoo _ _ hr := _root_.trans (symm_of r hr) hr
 
-instance [IsSymm α r] [foo r] : foo (flip r) where
+instance [IsSymm α r] [foo r] : foo rᵀ where
   isfoo _ _ h := by
     rw [Symmetric.flip_eq IsSymm.symm] at h ⊢
     exact refl_of_right h
@@ -404,28 +516,32 @@ lemma transClosure_self_iff [foo r] : TransClosure r a a ↔ r a a := by
   · exact h
   exact refl_of_right h
 
+instance [IsSymm α r] [IsTrans α r] : Domple r where
+  domple := by
+    rintro a b ⟨c, ⟨d, had, hcd⟩, hcb⟩
+    exact trans' had (trans' (symm hcd) hcb)
 
 
-def reflSet (r : α → α → Prop) : Set α := {x | r x x}
+-- def reflSet (r : α → α → Prop) : Set α := {x | r x x}
 
-@[simp]
-lemma mem_reflSet_iff (r : α → α → Prop) : a ∈ reflSet r ↔ r a a := Iff.rfl
+-- @[simp]
+-- lemma mem_reflSet_iff (r : α → α → Prop) : a ∈ reflSet r ↔ r a a := Iff.rfl
 
-lemma reflSet_eq_refl (r : α → α → Prop) : reflSet r = {x | r x x} := rfl
+-- lemma reflSet_eq_refl (r : α → α → Prop) : reflSet r = {x | r x x} := rfl
 
-lemma sup_reflSet (r s : α → α → Prop) : reflSet (r ⊔ s) = reflSet r ⊔ reflSet s := rfl
+-- lemma sup_reflSet (r s : α → α → Prop) : reflSet (r ⊔ s) = reflSet r ⊔ reflSet s := rfl
 
-lemma inf_reflSet (r s : α → α → Prop) : reflSet (r ⊓ s) = reflSet r ⊓ reflSet s := rfl
+-- lemma inf_reflSet (r s : α → α → Prop) : reflSet (r ⊓ s) = reflSet r ⊓ reflSet s := rfl
 
-lemma reflSet_eq_domain (r : α → α → Prop) [foo <| flip r] : reflSet r = domain r := by
-  ext a
-  rw [mem_reflSet_iff, mem_domain_iff]
-  exact ⟨fun h => ⟨a, h⟩, fun ⟨b, h⟩ => refl_of_left h⟩
+-- lemma reflSet_eq_domain (r : α → α → Prop) [foo <| flip r] : reflSet r = domain r := by
+--   ext a
+--   rw [mem_reflSet_iff, mem_domain_iff]
+--   exact ⟨fun h => ⟨a, h⟩, fun ⟨b, h⟩ => refl_of_left h⟩
 
-lemma reflSet_eq_codomain (r : α → α → Prop) [foo r] : reflSet r = codomain r := by
-  ext a
-  rw [mem_reflSet_iff, mem_codomain_iff]
-  exact ⟨fun h => ⟨a, h⟩, fun ⟨b, h⟩ => refl_of_right h⟩
+-- lemma reflSet_eq_codomain (r : α → α → Prop) [foo r] : reflSet r = codomain r := by
+--   ext a
+--   rw [mem_reflSet_iff, mem_codomain_iff]
+--   exact ⟨fun h => ⟨a, h⟩, fun ⟨b, h⟩ => refl_of_right h⟩
 
 
 
@@ -445,7 +561,7 @@ lemma comp_idem_right (r : α → α → Prop) [IsTrans α r] [foo <| flip r] (s
   ext x y
   refine ⟨fun ⟨a, ⟨b, hxb, hrba⟩, hray⟩ => ⟨b, hxb,  trans_of r hrba hray⟩,
     fun ⟨a, hxa, hray⟩ => ⟨a, ⟨a, hxa, ?_⟩, hray⟩⟩
-  change (flip r) a a
+  change rᵀ a a
   exact refl_of_right hray
 
 lemma comp_self (r : α → α → Prop) [IsTrans α r] [foo r] : Comp r r = r := by
@@ -465,11 +581,11 @@ lemma restrict_mono {r s : α → α → Prop} (h : r ≤ s) (S : Set α) :
   rintro x y ⟨hr, hx, hy⟩
   exact ⟨h _ _ hr, hx, hy⟩
 
-lemma restrict_reflSet_subset (r : α → α → Prop) (S : Set α) : reflSet (restrict r S) ⊆ S :=
-  fun _ ⟨_, hx, _⟩ => hx
+-- lemma restrict_reflSet_subset (r : α → α → Prop) (S : Set α) : reflSet (restrict r S) ⊆ S :=
+--   fun _ ⟨_, hx, _⟩ => hx
 
-lemma restrict_reflSet_subset_reflSet (r : α → α → Prop) (S : Set α) :
-    reflSet (restrict r S) ⊆ reflSet r := fun _ ⟨hr, _, _⟩ => hr
+-- lemma restrict_reflSet_subset_reflSet (r : α → α → Prop) (S : Set α) :
+--     reflSet (restrict r S) ⊆ reflSet r := fun _ ⟨hr, _, _⟩ => hr
 
 lemma restrict_le (r : α → α → Prop) (S : Set α) : restrict r S ≤ r :=
   fun _ _ hrr => hrr.1
@@ -477,193 +593,64 @@ lemma restrict_le (r : α → α → Prop) (S : Set α) : restrict r S ≤ r :=
 lemma restrict_subset (r : α → α → Prop) {S T : Set α} (h : S ⊆ T) :
     restrict r S ≤ restrict r T := fun _ _ ⟨hr, hx, hy⟩ => ⟨hr, h hx, h hy⟩
 
-lemma restrict_eq_iff (r : α → α → Prop) [foo r] [foo <| flip r] (S : Set α) :
-    restrict r S = r ↔ reflSet r ⊆ S := by
-  refine ⟨fun hr x hx => ?_, fun h => ?_⟩
-  · rw [← hr, mem_reflSet_iff] at hx
-    exact hx.left_mem
-  · ext x y
-    simp only [restrict, and_iff_left_iff_imp]
-    exact fun hxy => ⟨h <| refl_of_left hxy, h <| refl_of_right hxy⟩
+-- lemma restrict_eq_iff (r : α → α → Prop) [foo r] [foo <| flip r] (S : Set α) :
+--     restrict r S = r ↔ reflSet r ⊆ S := by
+--   refine ⟨fun hr x hx => ?_, fun h => ?_⟩
+--   · rw [← hr, mem_reflSet_iff] at hx
+--     exact hx.left_mem
+--   · ext x y
+--     simp only [restrict, and_iff_left_iff_imp]
+--     exact fun hxy => ⟨h <| refl_of_left hxy, h <| refl_of_right hxy⟩
 
 
 
-def PER (α : Type*) := {r : α → α → Prop // IsSymm α r ∧ IsTrans α r}
+-- def comply (r : PER α) (s : α → α → Prop) : α → α → Prop :=
+--   Comp (Comp r s) r
 
-namespace PER
+-- lemma comply_mono (r : PER α) {s t : α → α → Prop} (hst : s ≤ t) :
+--     comply r s ≤ comply r t := by
+--   rintro x y h'
+--   let ⟨u, ⟨v, hxy, havu⟩, huy⟩ := h'
+--   exact ⟨u, ⟨v, hxy, hst _ _ havu⟩, huy ⟩
 
-variable {r' s' : PER α}
+-- @[simp]
+-- lemma comply_idem (r : PER α) (s : α → α → Prop) :
+--     comply r (comply r s) = comply r s := by
+--   unfold comply
+--   rw [comp_assoc, comp_idem_right, comp_assoc, comp_idem_left]
 
-instance : FunLike (PER α) α (α → Prop) where
-  coe := Subtype.val
-  coe_injective' := Subtype.val_injective
+-- @[simp]
+-- lemma comply_comp_left (r : PER α) (s : α → α → Prop) :
+--     Comp r (comply r s) = comply r s := by
+--   unfold comply
+--   rw [comp_assoc, comp_idem_left]
 
-@[ext] lemma ext {r s : PER α} (h : ⇑r = ⇑s) : r = s :=
-  instFunLikeForallProp.coe_injective.eq_iff.mp h
+-- @[simp]
+-- lemma comply_comp_right (r : PER α) (s : α → α → Prop) : Comp (comply r s) r = comply r s := by
+--   unfold comply
+--   rw [comp_assoc, comp_self]
 
-instance : IsSymm α r' := r'.property.1
-instance : IsTrans α r' := r'.property.2
-instance : IsSymm α r'.val := r'.property.1
-instance : IsTrans α r'.val := r'.property.2
-instance : PartialOrder (PER α) := Subtype.partialOrder _
-instance : OrderTop (PER α) := Subtype.orderTop ⟨inferInstance, inferInstance⟩
-instance : OrderBot (PER α) := Subtype.orderBot ⟨inferInstance, inferInstance⟩
-instance : CompleteLattice (PER α) where
-  sup r s := ⟨TransClosure (r ⊔ s), inferInstance, inferInstance⟩
-  le_sup_left r s := by
-    change r ≤ TransClosure (r ⊔ s)
-    exact le_trans le_sup_left (TransClosure.le_closure _)
-  le_sup_right r s := by
-    change s ≤ TransGen (r ⊔ s)
-    exact le_trans le_sup_right (TransClosure.le_closure _)
-  sup_le r s t hrt hst := by
-    change TransClosure (r ⊔ s) ≤ t
-    exact ClosureOperator.closure_min (sup_le hrt hst) t.prop.2.trans
-  inf r s := ⟨r ⊓ s, inferInstance, inferInstance⟩
-  inf_le_left r s := by
-    change r.val ⊓ s ≤ r
-    exact inf_le_left
-  inf_le_right r s := by
-    change r.val ⊓ s ≤ s
-    exact inf_le_right
-  le_inf r s t hrt hst := by
-    change r ≤ s.val ⊓ t
-    exact le_inf hrt hst
-  sSup s := ⟨TransGen (sSup <| Subtype.val '' s),
-    @instIsSymmCoeClosureOperatorForallForallPropTransClosure _ _
-    <| sSup_symm (s := Subtype.val '' s) (fun r ⟨r', hr', heq⟩ => heq ▸ r'.prop.1), inferInstance⟩
-  le_sSup S r hrS := by
-    change r ≤ TransGen (sSup <| Subtype.val '' S)
-    exact le_trans (le_sSup <| mem_image_of_mem Subtype.val hrS) (TransClosure.le_closure _)
-  sSup_le S r hrS := by
-    refine TransClosure.closure_min (sSup_le ?_) r.prop.2.trans
-    rintro s ⟨s', hs', rfl⟩
-    exact hrS s' hs'
-  sInf S := ⟨sInf <| Subtype.val '' S, sInf_symm (fun r ⟨r', hr', heq⟩ => heq ▸ r'.prop.1),
-    sInf_trans (fun r ⟨r', hr', heq⟩ => heq ▸ r'.prop.2)⟩
-  le_sInf S r hrS := by
-    change r ≤ sInf (Subtype.val '' S)
-    refine le_sInf <| ?_
-    rintro s ⟨s', hs', rfl⟩
-    exact hrS s' hs'
-  sInf_le S r hrS := sInf_le <| mem_image_of_mem Subtype.val hrS
-  le_top r := by simp
-  bot_le r := by simp
+-- lemma comply_reflset_mono {r : PER α} {s₁ s₂ : α → α → Prop} (h₁ : s₁ ≤ s₂) :
+--     reflSet (comply r s₁) ≤ reflSet (comply r s₂) :=
+--   fun _ ⟨u, ⟨v, huv, hvx⟩, huy⟩ => ⟨u, ⟨v, huv, h₁ _ _ hvx⟩, huy⟩
 
-@[simp]
-lemma sup_reflSet (r s : PER α) : reflSet (r ⊔ s : PER α) = reflSet r ⊔ reflSet s := by
-  ext x
-  change TransClosure (r ⊔ s) x x ↔ _
-  rw [transClosure_self_iff]
-  simp only [Pi.sup_apply, sup_Prop_eq, sup_eq_union, mem_union, mem_reflSet_iff]
+-- lemma comply_reflset_subset (r : PER α) (s : α → α → Prop) : reflSet (comply r s) ⊆ reflSet r :=
+--   fun _ ⟨_, ⟨_, huv, _⟩, _⟩ => refl_of_left huv
 
-@[simp]
-lemma inf_reflSet (r s : PER α) : reflSet (r ⊓ s : PER α) = reflSet r ⊓ reflSet s := rfl
+-- lemma comply_mono_left (hrs : r ≤ s) (s₁ : α → α → Prop) : comply r s₁ ≤ comply s s₁ :=
+--   fun _ _ ⟨u, ⟨v, hxy, havu⟩, huy⟩ => ⟨u, ⟨v, hrs _ _ hxy, havu⟩, hrs _ _ huy⟩
 
-@[simp]
-lemma sSup_reflSet (s : Set (PER α)) :
-    reflSet (sSup s : PER α) = ⋃₀ ((reflSet ∘ Subtype.val) '' s) := by
-  ext x
-  change TransClosure _ x x ↔ _
-  have := foo_sSup (s := Subtype.val '' s) (fun r ⟨r', hr', heq⟩ => heq ▸ inferInstance)
-  rw [transClosure_self_iff]
-  simp
+-- lemma restrict_reflSet_le_comply (r : PER α) (s : α → α → Prop) :
+--     restrict s (reflSet r) ≤ comply r s :=
+--   fun x y ⟨hxy, hx, hy⟩ => ⟨y, ⟨x, hx, hxy⟩, hy⟩
 
-@[simp]
-lemma sInf_reflSet (s : Set (PER α)) :
-    reflSet (sInf s : PER α) = ⋂₀ ((reflSet ∘ Subtype.val) '' s) := by
-  ext x
-  have := foo_sInf (s := Subtype.val '' s) (fun r ⟨r', hr', heq⟩ => heq ▸ inferInstance)
-  change sInf (Subtype.val '' s) x x ↔ _
-  simp only [sInf_apply, iInf_apply, iInf_Prop_eq, Subtype.forall, mem_image, Subtype.exists,
-    exists_and_right, exists_eq_right, forall_exists_index, comp_apply, mem_sInter, and_imp]
-  refine ⟨fun h S r hr hrs heq => ?_, fun h r hr hrs => h (reflSet r) r hr hrs rfl⟩
-  subst heq
-  exact (mem_reflSet_iff r).mpr (h r hr hrs)
+-- @[simp]
+-- lemma restrict_comply_eq_comply (r : PER α) (s : α → α → Prop) :
+--     comply r (restrict s (reflSet r)) = comply r s := by
+--   ext x y
+--   exact ⟨fun ⟨u, ⟨v, hxv, hsvu, hv, hu⟩, huy⟩ => ⟨u, ⟨v, hxv, hsvu⟩, huy⟩,
+--     fun ⟨u, ⟨v, hxv, hsvu⟩, huy⟩ => ⟨u, ⟨v, hxv, hsvu, refl_of_right hxv, refl_of_left huy⟩, huy⟩⟩
 
-variable {r s : PER α}
-
-lemma fiber_eq_fiber_iff (hx : r a a) : fiber r a = fiber r b ↔ r a b := by
-  refine ⟨fun h => ?_, fun h => ?_⟩
-  · simp only [Set.ext_iff, mem_fiber_iff] at h
-    exact h a |>.1 (symm hx)
-  ext _
-  exact rel_congr_right h
-
-lemma fiber_eq_fiber (hxy : r a b) : fiber r a = fiber r b :=
-  fiber_eq_fiber_iff (refl_of_left hxy) |>.2 hxy
-
-instance : HasSubset (PER α) where
-  Subset r s := fibers r ⊆ fibers s
-
-lemma le_of_subset {r s : PER α} (h : r ⊆ s) : r ≤ s := by
-  rintro a b hr
-  obtain ⟨c, hc, heq⟩ := h <| fiber_mem_fibers hr
-  have ha : a ∈ fiber r b := hr
-  have hb : b ∈ fiber r b := refl_of_right hr
-  rw [← heq] at ha hb
-  exact trans' ha (symm hb)
-
-instance : IsPartialOrder (PER α) (· ⊆ ·) where
-  refl _ _ := id
-  antisymm _ _ h₁ h₂ := le_antisymm (le_of_subset h₁) (le_of_subset h₂)
-  trans _ _ _ h₁ h₂ _ a := h₂ (h₁ a)
-
-lemma fibers_inj (h : fibers r = fibers s) : r = s :=
-  le_antisymm (le_of_subset h.subset) (le_of_subset h.superset)
-
-
-
-def comply (r : PER α) (s : α → α → Prop) : α → α → Prop :=
-  Comp (Comp r s) r
-
-lemma comply_mono (r : PER α) {s t : α → α → Prop} (hst : s ≤ t) :
-    comply r s ≤ comply r t := by
-  rintro x y h'
-  let ⟨u, ⟨v, hxy, havu⟩, huy⟩ := h'
-  exact ⟨u, ⟨v, hxy, hst _ _ havu⟩, huy ⟩
-
-@[simp]
-lemma comply_idem (r : PER α) (s : α → α → Prop) :
-    comply r (comply r s) = comply r s := by
-  unfold comply
-  rw [comp_assoc, comp_idem_right, comp_assoc, comp_idem_left]
-
-@[simp]
-lemma comply_comp_left (r : PER α) (s : α → α → Prop) :
-    Comp r (comply r s) = comply r s := by
-  unfold comply
-  rw [comp_assoc, comp_idem_left]
-
-@[simp]
-lemma comply_comp_right (r : PER α) (s : α → α → Prop) : Comp (comply r s) r = comply r s := by
-  unfold comply
-  rw [comp_assoc, comp_self]
-
-lemma comply_reflset_mono {r : PER α} {s₁ s₂ : α → α → Prop} (h₁ : s₁ ≤ s₂) :
-    reflSet (comply r s₁) ≤ reflSet (comply r s₂) :=
-  fun _ ⟨u, ⟨v, huv, hvx⟩, huy⟩ => ⟨u, ⟨v, huv, h₁ _ _ hvx⟩, huy⟩
-
-lemma comply_reflset_subset (r : PER α) (s : α → α → Prop) : reflSet (comply r s) ⊆ reflSet r :=
-  fun _ ⟨_, ⟨_, huv, _⟩, _⟩ => refl_of_left huv
-
-lemma comply_mono_left (hrs : r ≤ s) (s₁ : α → α → Prop) : comply r s₁ ≤ comply s s₁ :=
-  fun _ _ ⟨u, ⟨v, hxy, havu⟩, huy⟩ => ⟨u, ⟨v, hrs _ _ hxy, havu⟩, hrs _ _ huy⟩
-
-lemma restrict_reflSet_le_comply (r : PER α) (s : α → α → Prop) :
-    restrict s (reflSet r) ≤ comply r s :=
-  fun x y ⟨hxy, hx, hy⟩ => ⟨y, ⟨x, hx, hxy⟩, hy⟩
-
-@[simp]
-lemma restrict_comply_eq_comply (r : PER α) (s : α → α → Prop) :
-    comply r (restrict s (reflSet r)) = comply r s := by
-  ext x y
-  exact ⟨fun ⟨u, ⟨v, hxv, hsvu, hv, hu⟩, huy⟩ => ⟨u, ⟨v, hxv, hsvu⟩, huy⟩,
-    fun ⟨u, ⟨v, hxv, hsvu⟩, huy⟩ => ⟨u, ⟨v, hxv, hsvu, refl_of_right hxv, refl_of_left huy⟩, huy⟩⟩
-
-lemma comply_le {s t : α → α → Prop} (h1 : restrict s (reflSet r) ≤ t)
-    (h2 : comply r t ≤ t) : comply r s ≤ t :=
-  (restrict_comply_eq_comply r _) ▸ comply_mono r h1 |>.trans h2
-
-end PER
-end Relation
+-- lemma comply_le {s t : α → α → Prop} (h1 : restrict s (reflSet r) ≤ t)
+--     (h2 : comply r t ≤ t) : comply r s ≤ t :=
+--   (restrict_comply_eq_comply r _) ▸ comply_mono r h1 |>.trans h2
