Matroid/ForMathlib/SetPartition.lean
@@ -1,32 +1,29 @@
 import Mathlib.Data.Setoid.Partition
 import Mathlib.Data.SetLike.Basic
 import Mathlib.Data.Set.Finite.Powerset
-import Mathlib.Data.PFun
-import Mathlib.Order.Closure
 import Matroid.ForMathlib.Lattice
+import Matroid.ForMathlib.Relation
 
-open Set Function
+open Set Function Relation
 
 variable {α β : Type*} {s t x y z : α}
 
-structure Partition [CompleteLattice α] (s : α) where
+structure Partition (α : Type*) [CompleteLattice α] where
   parts : Set α
   indep : sSupIndep parts
   bot_notMem : ⊥ ∉ parts
-  sSup_eq' : sSup parts = s
 
 namespace Partition
 
 section Basic
 
-variable [CompleteLattice α] {P Q : Partition s}
+variable [CompleteLattice α] {P Q : Partition α}
 
-instance : SetLike (Partition s) α where
+def supp (P : Partition α) : α := sSup P.parts
+
+instance : SetLike (Partition α) α where
   coe := Partition.parts
   coe_injective' p p' h := by cases p; cases p'; simpa using h
-
-instance : HasSubset (Partition s) where
-  Subset P Q := P.parts ⊆ Q.parts
 
 @[simp] lemma mem_parts : x ∈ P.parts ↔ x ∈ (P : Set α) := Iff.rfl
 
@@ -36,6 +33,14 @@ instance : HasSubset (Partition s) where
   simp only [mk.injEq]
   ext x
   simpa using hP x
+
+instance : HasSubset (Partition α) where
+  Subset P Q := P.parts ⊆ Q.parts
+
+instance : IsPartialOrder (Partition (Set α)) (· ⊆ ·) where
+  refl _ _ := id
+  trans _ _ _ hPQ hQR _ h := hQR (hPQ h)
+  antisymm _ _ hPQ hPQ' := by ext S; exact ⟨(hPQ ·), (hPQ' ·)⟩
 
 lemma disjoint (hx : x ∈ P) (hy : y ∈ P) (hxy : x ≠ y) : Disjoint x y :=
   P.indep.pairwiseDisjoint hx hy hxy
@@ -49,33 +54,17 @@ lemma ne_bot_of_mem (hx : x ∈ P) : x ≠ ⊥ :=
 lemma bot_lt_of_mem (hx : x ∈ P) : ⊥ < x :=
   bot_lt_iff_ne_bot.2 <| P.ne_bot_of_mem hx
 
-lemma iSup_eq (P : Partition s) : ⨆ x ∈ P, x = s := by
-  simp_rw [← P.sSup_eq', sSup_eq_iSup]
+lemma sSup_eq (P : Partition α) : sSup P = P.supp  := rfl
+
+lemma iSup_eq (P : Partition α) : ⨆ x ∈ P, x = P.supp := by
+  simp_rw [← P.sSup_eq, sSup_eq_iSup]
   rfl
 
-lemma sSup_eq (P : Partition s) : sSup P = s :=
-  P.sSup_eq'
-
-lemma le_of_mem (P : Partition s) (hx : x ∈ P) : x ≤ s :=
+lemma le_of_mem (P : Partition α) (hx : x ∈ P) : x ≤ P.supp :=
   (le_sSup hx).trans_eq P.sSup_eq
 
-lemma parts_nonempty (P : Partition s) (hs : s ≠ ⊥) : (P : Set α).Nonempty :=
+lemma parts_nonempty (P : Partition α) (hs : P.supp ≠ ⊥) : (P : Set α).Nonempty :=
   nonempty_iff_ne_empty.2 fun hP ↦ by simp [← P.sSup_eq, hP, sSup_empty] at hs
-
-@[simps] protected def congr (P : Partition s) (hst : s = t) : Partition t where
-  parts := P.parts
-  indep := P.indep
-  bot_notMem := P.bot_notMem
-  sSup_eq' := hst ▸ P.sSup_eq'
-
-@[simp] lemma coe_congr_eq (hst : s = t) :
-    (P.congr hst : Set α) = P := rfl
-
-@[simp] lemma mem_congr_iff (hst : s = t) :
-    x ∈ P.congr hst ↔ x ∈ P := Iff.rfl
-
-@[simps!] def partsCongrEquiv (P : Partition s) (hst : s = t) :
-    (P : Set α) ≃ (P.congr hst : Set α) := Equiv.setCongr rfl
 
 end Basic
 
@@ -83,23 +72,35 @@ section PairwiseDisjoint
 
 variable {α : Type*} [Order.Frame α] {s t x y z : α} {parts : Set α}
 
-@[simps] def ofPairwiseDisjoint (h : parts.PairwiseDisjoint id) (h_empty : ⊥ ∉ parts):
-    Partition (sSup parts) where
+@[simps] def ofPairwiseDisjoint (pairwiseDisjoint : parts.PairwiseDisjoint id)
+    (forall_nonempty : ⊥ ∉ parts) : Partition α where
   parts := parts
-  indep := sSupIndep_iff_pairwiseDisjoint.mpr h
-  bot_notMem := h_empty
-  sSup_eq' := rfl
+  indep := sSupIndep_iff_pairwiseDisjoint.mpr pairwiseDisjoint
+  bot_notMem := forall_nonempty
+
+@[simp] lemma mem_ofPairwiseDisjoint (pairwiseDisjoint : parts.PairwiseDisjoint id)
+    (forall_nonempty : ⊥ ∉ parts) :
+  x ∈ ofPairwiseDisjoint pairwiseDisjoint forall_nonempty ↔ x ∈ parts := Iff.rfl
+
+@[simp]
+lemma supp_ofPairwiseDisjoint (pairwiseDisjoint : parts.PairwiseDisjoint id)
+    (forall_nonempty : ⊥ ∉ parts) :
+  (ofPairwiseDisjoint pairwiseDisjoint forall_nonempty).supp = sSup parts := rfl
 
 @[simps] def ofPairwiseDisjoint' (pairwiseDisjoint : parts.PairwiseDisjoint id)
-  (forall_nonempty : ∀ s ∈ parts, s ≠ ⊥) (eq_sUnion : s = sSup parts) :
-    Partition s where
+  (forall_nonempty : ∀ s ∈ parts, s ≠ ⊥) :
+    Partition α where
   parts := parts
   indep := pairwiseDisjoint.sSupIndep
   bot_notMem := fun h ↦ by simpa using forall_nonempty _ h
-  sSup_eq' := eq_sUnion.symm
 
-@[simp] lemma mem_ofPairwiseDisjoint' (pairwiseDisjoint) (forall_nonempty) (eq_sUnion) {x : α} :
-  x ∈ ofPairwiseDisjoint' (s := s) (parts := parts) pairwiseDisjoint forall_nonempty eq_sUnion ↔
+@[simp]
+lemma supp_ofPairwiseDisjoint' (pairwiseDisjoint : parts.PairwiseDisjoint id)
+    (forall_nonempty : ∀ s ∈ parts, s ≠ ⊥) :
+  (ofPairwiseDisjoint' pairwiseDisjoint forall_nonempty).supp = sSup parts := rfl
+
+@[simp] lemma mem_ofPairwiseDisjoint' (pairwiseDisjoint) (forall_nonempty) {x : α} :
+  x ∈ ofPairwiseDisjoint' (parts := parts) pairwiseDisjoint forall_nonempty ↔
     x ∈ parts := Iff.rfl
 
 end PairwiseDisjoint
@@ -109,29 +110,46 @@ section indep
 variable [CompleteLattice α] {u : Set α} {a : α}
 
 /-- A `sSupIndep` collection not containing `⊥` gives a partition of its supremum. -/
-@[simps] def ofIndependent (hs : sSupIndep u) (hbot : ⊥ ∉ u) :
-    Partition (sSup u) where
+@[simps] def ofIndependent {u : Set α} (hs : sSupIndep u) (hbot : ⊥ ∉ u) : Partition α where
   parts := u
   indep := hs
   bot_notMem := hbot
-  sSup_eq' := rfl
 
-@[simp] lemma mem_ofIndependent_iff (hu : sSupIndep u) (h : ⊥ ∉ u) :
-    a ∈ ofIndependent hu h ↔ a ∈ u := Iff.rfl
+@[simp] lemma mem_ofIndependent_iff {u : Set α} (hu : sSupIndep u)
+    (h : ⊥ ∉ u) {a : α} : a ∈ ofIndependent hu h ↔ a ∈ u := Iff.rfl
+
+@[simp] lemma supp_ofIndependent {u : Set α} (hu : sSupIndep u) (hbot : ⊥ ∉ u) :
+    (ofIndependent hu hbot).supp = sSup u := rfl
 
 /-- A `sSupIndep` collection gives a partition of its supremum by removing `⊥`. -/
-def ofIndependent' (hs : sSupIndep u) : Partition (sSup u) :=
-  (ofIndependent (hs.mono (diff_subset (t := {⊥}))) (fun h ↦ h.2 rfl)).congr (by simp)
+def ofIndependent' {u : Set α} (hs : sSupIndep u) : Partition α :=
+  (ofIndependent (hs.mono (diff_subset (t := {⊥}))) (fun h ↦ h.2 rfl))
 
-@[simp] lemma mem_ofIndependent'_iff (hu : sSupIndep u) :
+@[simp] lemma mem_ofIndependent'_iff {u : Set α} (hu : sSupIndep u) {a : α} :
   a ∈ ofIndependent' hu ↔ a ∈ u ∧ a ≠ ⊥ := Iff.rfl
 
+@[simp] lemma supp_ofIndependent' {u : Set α} (hu : sSupIndep u) :
+    (ofIndependent' hu).supp = sSup u := by
+  show sSup (u \ {⊥}) = sSup u
+  simp
+
+/-- The subpartition with over a subset of the parts. -/
+def restrict {P : Partition α} {s : Set α} (hs : s ⊆ P.parts) : Partition α where
+  parts := s
+  indep := P.indep.mono hs
+  bot_notMem h := P.bot_notMem (hs h)
+
+@[simp] lemma restrict_parts {P : Partition α} {s : Set α} (hs : s ⊆ P.parts) :
+    (P.restrict hs).parts = s := rfl
+
+@[simp] lemma mem_restrict_iff {P : Partition α} {s : Set α} (hs : s ⊆ P.parts) {a : α} :
+    a ∈ P.restrict hs ↔ a ∈ s := Iff.rfl
+
 /-- The partition with no parts. -/
-@[simps] protected def empty (α : Type*) [CompleteLattice α] : Partition (⊥ : α) where
+@[simps] protected def empty (α : Type*) [CompleteLattice α] : Partition α where
   parts := ∅
   indep := by simp
   bot_notMem := by simp
-  sSup_eq' := by simp
 
 @[simp] lemma empty_coe_eq (α : Type*) [CompleteLattice α] :
     (Partition.empty α : Set α) = ∅ := rfl
@@ -141,39 +159,59 @@ def ofIndependent' (hs : sSupIndep u) : Partition (sSup u) :=
   rw [← SetLike.mem_coe, empty_coe_eq]
   simp
 
-lemma eq_empty (P : Partition (⊥ : α)) : P = Partition.empty α := by
+@[simp] lemma supp_empty (α : Type*) [CompleteLattice α] : (Partition.empty α).supp = ⊥ := by
+  simp [Partition.empty, supp]
+
+lemma eq_empty {P : Partition α} (hP : P.supp = ⊥) : P = Partition.empty α := by
   ext x
   have hsup := P.sSup_eq
-  simp only [sSup_eq_bot, SetLike.mem_coe] at hsup
+  simp only [sSup_eq_bot, SetLike.mem_coe, hP] at hsup
   simp only [notMem_empty, iff_false]
   exact fun hx ↦ P.ne_bot_of_mem hx <| hsup x hx
 
-instance : Unique (Partition (⊥ : α)) where
+@[simp]
+lemma supp_eq_bot_iff {P : Partition α} : P.supp = ⊥ ↔ P = Partition.empty α := by
+  refine ⟨eq_empty, ?_⟩
+  rintro rfl
+  exact supp_empty α
+
+instance {α : Type*} [CompleteLattice α] [Subsingleton α] : Unique (Partition α) where
   default := Partition.empty α
-  uniq := by simp [eq_empty]
+  uniq P := eq_empty (by
+    simp only [← P.sSup_eq, sSup_eq_bot, SetLike.mem_coe]
+    exact fun a b ↦ Subsingleton.elim _ _)
 
 /-- The one-part partition. -/
-@[simps] def indiscrete (s : α) (hs : s ≠ ⊥) : Partition s where
+@[simps] def indiscrete (s : α) (hs : s ≠ ⊥) : Partition α where
   parts := {s}
   indep := by simp [sSupIndep]
   bot_notMem := by simpa using hs.symm
-  sSup_eq' := sSup_singleton
 
-@[simp] lemma mem_indiscrete_iff (s : α) (hs : s ≠ ⊥) :
+@[simp] lemma mem_indiscrete_iff (s : α) (hs : s ≠ ⊥) {a : α} :
     a ∈ Partition.indiscrete s hs ↔ a = s := Iff.rfl
 
-noncomputable def indiscrete' (s : α) : Partition s :=
+@[simp]
+lemma supp_indiscrete (s : α) (hs : s ≠ ⊥) : (Partition.indiscrete s hs).supp = s := by
+  simp [Partition.indiscrete, supp]
+
+noncomputable def indiscrete' (s : α) : Partition α :=
   let _ : Decidable (s = ⊥) := Classical.dec _
-  if hs : s = ⊥ then (Partition.empty α).congr hs.symm else indiscrete s hs
+  if hs : s = ⊥ then Partition.empty α else indiscrete s hs
 
 @[simp]
-lemma indiscrete'_eq_empty : indiscrete' ⊥ = (Partition.empty α) := by
-  simp only [indiscrete', ↓reduceDIte]
-  rfl
+lemma indiscrete'_eq_empty : indiscrete' ⊥ = Partition.empty α := by
+  simp [indiscrete']
 
 @[simp]
-lemma indiscrete'_eq_of_ne_bot (hs : s ≠ ⊥) : indiscrete' s = indiscrete s hs := by
+lemma indiscrete'_eq_of_ne_bot {s : α} (hs : s ≠ ⊥) : indiscrete' s = indiscrete s hs := by
   simp only [indiscrete', hs, ↓reduceDIte]
+
+@[simp]
+lemma supp_indiscrete' {s : α} : (indiscrete' s).supp = s := by
+  simp [indiscrete']
+  split_ifs with hs
+  · rw [supp_empty, hs]
+  · rw [supp_indiscrete s hs]
 
 @[simp]
 lemma mem_indiscrete'_iff : a ∈ indiscrete' s ↔ a = s ∧ a ≠ ⊥ := by
@@ -199,7 +237,7 @@ section Order
 
 variable {α : Type*} [CompleteLattice α] {s t a : α}
 
-instance : PartialOrder (Partition s) where
+instance : PartialOrder (Partition α) where
   le P Q := ∀ x ∈ P, ∃ y ∈ Q, x ≤ y
   lt := _
   le_refl P x hx := by
@@ -221,28 +259,36 @@ instance : PartialOrder (Partition s) where
       (hxy.trans hyx')
     rwa [hxy.antisymm hyx']
 
-instance : OrderTop (Partition s) where
-  top := (ofIndependent' (sSupIndep_singleton s)).congr sSup_singleton
+instance : OrderTop (Partition α) where
+  top := ofIndependent' (sSupIndep_singleton ⊤)
   le_top := by
-    obtain (rfl | hs) := eq_or_ne s ⊥
-    · simp
-    rintro P x hx
-    refine ⟨s, ?_, P.le_of_mem hx⟩
-    change s ∈ Partition.congr _ _
-    rw [mem_congr_iff, mem_ofIndependent'_iff]
-    exact ⟨rfl, hs⟩
+    obtain (hs | hs) := eq_or_ne ⊤ (⊥ : α)
+    · have : Subsingleton α := subsingleton_of_bot_eq_top hs.symm
+      simp [hs]
+    exact fun P x hx ↦ ⟨⊤, by simp [hs], by simp⟩
 
-@[simp] lemma mem_top_iff : a ∈ (⊤ : Partition s) ↔ a = s ∧ a ≠ ⊥ := by
-  change a ∈ Partition.congr _ _ ↔ _
-  rw [mem_congr_iff, mem_ofIndependent'_iff, mem_singleton_iff]
+@[simp] lemma mem_top_iff {a : α} : a ∈ (⊤ : Partition α) ↔ a = ⊤ ∧ a ≠ ⊥ := by
+  change a ∈ ofIndependent' (sSupIndep_singleton ⊤) ↔ _
+  rw [mem_ofIndependent'_iff, mem_singleton_iff]
 
-lemma top_eq_indiscrete (hs : s ≠ ⊥) : (⊤ : Partition s) = indiscrete s hs := by
+lemma top_eq_indiscrete (hs : ⊤ ≠ ⊥) : (⊤ : Partition α) = indiscrete ⊤ hs := by
   ext a
   rw [mem_top_iff, mem_indiscrete_iff, and_iff_left_iff_imp]
   rintro rfl; assumption
 
-lemma parts_top_subset (s : α) : ((⊤ : Partition s) : Set α) ⊆ {s} := by
+lemma parts_top_subset : ((⊤ : Partition α) : Set α) ⊆ {⊤} := by
   simp
+
+instance : OrderBot (Partition α) where
+  bot := Partition.empty α
+  bot_le a s hs := by simp only [notMem_empty] at hs
+
+@[simp] lemma notMem_bot {a : α} : a ∉ (⊥ : Partition α) := notMem_empty α
+
+@[simp] lemma supp_bot : (⊥ : Partition α).supp = ⊥ := sSup_empty
+
+lemma supp_le_of_le {P Q : Partition α} (h : P ≤ Q) : P.supp ≤ Q.supp :=
+  sSup_le_sSup_of_forall_exists_le h
 
 end Order
 
@@ -251,21 +297,22 @@ section Discrete
 variable {α : Type*} [CompleteAtomicBooleanAlgebra α]
 
 /-- The discrete partition -/
-protected noncomputable def discrete (a : α) : Partition a :=
+protected noncomputable def discrete (a : α) : Partition α :=
   let S := {b : α | IsAtom b ∧ b ≤ a}
   have hSatom : ∀ b ∈ S, IsAtom b := by
     simp only [mem_setOf_eq, and_imp, S]
     tauto
   { parts := S
     indep := sSupIndep_atoms hSatom
-    bot_notMem h := by simpa using (hSatom ⊥ h).1
-    sSup_eq' := sSup_atoms_le_eq a}
+    bot_notMem h := by simpa using (hSatom ⊥ h).1}
+
+@[simp] lemma supp_discrete (a : α) : (Partition.discrete a).supp = a :=
+  sSup_atoms_le_eq a
 
 @[simp] lemma mem_discrete_iff {a b : α} : b ∈ Partition.discrete a ↔ IsAtom b ∧ b ≤ a := by rfl
 
-noncomputable instance {s : α} : OrderBot (Partition s) where
-  bot := Partition.discrete s
-  bot_le P _ hx := exists_mem_le_of_le_sSup_of_isAtom hx.1 hx.2 P.sSup_eq.ge
+-- lemma discrete_le_of_supp_eq (P : Partition α) : Partition.discrete P.supp ≤ P := by
+--   sorry
 
 end Discrete
 
@@ -273,53 +320,60 @@ section Bind
 
 variable {α : Type*} [CompleteDistribLattice α] {s : α}
 
-@[simps] protected def bind (P : Partition s) (Qs : ∀ a ∈ P, Partition a) : Partition s where
+@[simps] protected def bind (P : Partition α) (Qs : ∀ a ∈ P, Partition α)
+    (hQs : ∀ a, (h : a ∈ P) → (Qs a h).supp = a) : Partition α where
   parts := ⋃ a : P, (Qs a a.prop)
   indep := by
     intro b hb
     simp only [mem_iUnion, SetLike.mem_coe, Subtype.exists] at hb
     obtain ⟨a, haP, hba : b ∈ Qs a haP⟩ := hb
+    obtain hasupp := hQs a haP
     have hdj1 := (Qs a haP).indep hba
-    have hdj2 := (P.indep haP).mono_left <| (Qs a haP).le_of_mem hba
+    have hdj2 := (hasupp ▸ P.indep haP).mono_left <| (Qs a haP).le_of_mem hba
     refine (hdj1.sup_right hdj2).mono_right ?_
     simp only [mem_iUnion, SetLike.mem_coe, Subtype.exists, sSup_le_iff, mem_diff,
       mem_singleton_iff, and_imp, forall_exists_index]
 
     rintro t' x hx (ht' : t' ∈ Qs x hx) hne
+    obtain hxsupp := hQs x hx
     obtain (rfl | hne) := eq_or_ne x a
     · exact (le_sSup_of_le (show t' ∈ _ \ {b} from ⟨ht', hne⟩) rfl.le).trans le_sup_left
-    exact (le_sSup_of_le (show x ∈ P.parts \ ({a} : Set α) from ⟨hx, hne⟩)
-      ((Qs x hx).le_of_mem ht')).trans le_sup_right
+    refine le_trans (le_sSup_of_le ?_ ((Qs x hx).le_of_mem ht')) le_sup_right
+    simp [hasupp, hxsupp, hne, hx]
   bot_notMem := by
     simp only [mem_iUnion, SetLike.mem_coe, Subtype.exists, not_exists]
     exact fun x hx ↦ (Qs x hx).bot_notMem
-  sSup_eq' := by
-    simp_rw [sSup_iUnion, Partition.sSup_eq, ← P.sSup_eq, sSup_eq_iSup, iSup_subtype]; rfl
 
-@[simp] lemma mem_bind_iff {P : Partition s} {Qs : ∀ a ∈ P, Partition a} {a : α} :
-    a ∈ P.bind Qs ↔ ∃ (b : α) (hb : b ∈ P), a ∈ Qs b hb := by
+@[simp] lemma mem_bind_iff {P : Partition α} {Qs : ∀ a ∈ P, Partition α}
+    (hQs : ∀ a, (h : a ∈ P) → (Qs a h).supp = a) {a : α} :
+    a ∈ P.bind Qs hQs ↔ ∃ (b : α) (hb : b ∈ P), a ∈ Qs b hb := by
   change _ ∈ ⋃ _, _ ↔ _; simp
 
-@[simp] lemma bind_le {α : Type*} [CompleteDistribLattice α] {s : α} (P : Partition s)
-    (Qs : ∀ a ∈ P, Partition a) : P.bind Qs ≤ P := by
+@[simp] lemma bind_le {α : Type*} [CompleteDistribLattice α] (P : Partition α)
+    (Qs : ∀ a ∈ P, Partition α) (hQs : ∀ a, (h : a ∈ P) → (Qs a h).supp = a) :
+    P.bind Qs hQs ≤ P := by
   intro t ht
-  obtain ⟨b, hbp, h⟩ := mem_bind_iff.1 ht
-  exact ⟨b, hbp, Partition.le_of_mem _ h⟩
+  obtain ⟨b, hbp, h⟩ := (mem_bind_iff hQs).1 ht
+  exact ⟨b, hbp, (hQs b hbp) ▸ Partition.le_of_mem _ h⟩
 
 end Bind
 
 section Set
 
-variable {s t u : Set α} {P : Partition s} {x : α}
+variable {s t u : Set α} {P : Partition (Set α)} {x : α}
 
-@[simp] protected lemma sUnion_eq (P : Partition s) : ⋃₀ P = s :=
+@[simp] protected lemma sUnion_eq (P : Partition (Set α)) : ⋃₀ P = P.supp :=
   P.sSup_eq
 
 lemma nonempty_of_mem (ht : t ∈ P) : t.Nonempty :=
   notMem_singleton_empty.1 <| P.ne_bot_of_mem ht
 
-lemma subset_of_mem (ht : t ∈ P) : t ⊆ s :=
+lemma subset_of_mem (ht : t ∈ P) : t ⊆ P.supp :=
   P.le_of_mem ht
+
+lemma mem_supp_iff : x ∈ P.supp ↔ ∃ t ∈ P, x ∈ t := by
+  refine ⟨fun hx ↦ ?_, fun ⟨t, htP, hxt⟩ ↦ subset_of_mem htP hxt⟩
+  rwa [← P.sUnion_eq, mem_sUnion] at hx
 
 lemma eq_of_mem_inter (ht : t ∈ P) (hu : u ∈ P) (hx : x ∈ t ∩ u) : t = u :=
   PairwiseDisjoint.elim P.pairwiseDisjoint ht hu fun
@@ -328,292 +382,380 @@ lemma eq_of_mem_inter (ht : t ∈ P) (hu : u ∈ P) (hx : x ∈ t ∩ u) : t = u
 lemma eq_of_mem_of_mem (ht : t ∈ P) (hu : u ∈ P) (hxt : x ∈ t) (hxu : x ∈ u) : t = u :=
   eq_of_mem_inter ht hu ⟨hxt, hxu⟩
 
-lemma exists_unique_of_mem_set (P : Partition s) (hx : x ∈ s) : ∃! t, t ∈ P ∧ x ∈ t := by
+lemma exists_unique_of_mem_supp (hx : x ∈ P.supp) : ∃! t, t ∈ P ∧ x ∈ t := by
   rw [← P.sUnion_eq, mem_sUnion] at hx
   obtain ⟨t, hxt⟩ := hx
   exact ⟨t, hxt, fun u ⟨huP, hxu⟩ ↦ eq_of_mem_inter huP hxt.1 ⟨hxu, hxt.2⟩⟩
 
-/-- The part containing a given element of the set being partitioned. If `x ∉ s`, then `∅`.  -/
-def partOf (P : Partition s) (x : α) : Set α :=
-  ⋃₀ {t ∈ P | x ∈ t}
+lemma mem_supp_iff_unique : x ∈ P.supp ↔ ∃! t, t ∈ P ∧ x ∈ t :=
+  ⟨exists_unique_of_mem_supp, fun ⟨_, ⟨htP, hxt⟩, _⟩ ↦ subset_of_mem htP hxt⟩
 
-lemma partOf_mem (P : Partition s) (hx : x ∈ s) : P.partOf x ∈ P := by
-  obtain ⟨t, ⟨h', h⟩⟩ := P.exists_unique_of_mem_set hx
-  have hrw : {t | t ∈ P ∧ x ∈ t} = {t} := by
-    ext t'
-    simp only [mem_setOf_eq, mem_singleton_iff]
-    exact ⟨h t', by rintro rfl; exact h'⟩
-  rw [partOf, hrw, sUnion_singleton]
-  exact h'.1
+lemma subset_sUnion_and_mem_iff_mem {S : Set (Set α)} (hSP : S ⊆ P.parts) :
+    t ⊆ ⋃₀ S ∧ t ∈ P ↔ t ∈ S := by
+  refine ⟨fun ⟨htsu, htP⟩ ↦ ?_, fun htS ↦ ⟨subset_sUnion_of_mem htS, hSP htS⟩⟩
+  obtain ⟨x, hxt⟩ := nonempty_of_mem htP
+  obtain ⟨s, hsS, hxs⟩ := htsu hxt
+  obtain rfl := eq_of_mem_of_mem htP (hSP hsS) hxt hxs
+  exact hsS
 
-lemma partOf_eq_empty (P : Partition s) (hx : x ∉ s) : P.partOf x = ∅ := by
-  rw [← P.sUnion_eq] at hx
-  simp only [partOf, eq_empty_iff_forall_notMem, mem_sUnion, mem_setOf, not_exists, not_and,
-    and_imp]
-  exact fun y t ht hxt _ ↦ hx <| mem_sUnion_of_mem hxt ht
-
-lemma mem_partOf (P : Partition s) (hx : x ∈ s) : x ∈ P.partOf x := by
-  obtain ⟨_, ⟨h, -⟩⟩ := P.exists_unique_of_mem_set hx
-  exact mem_sUnion_of_mem h.2 h
-
-lemma eq_partOf_of_mem {P : Partition s} (ht : t ∈ P) (hxt : x ∈ t) :
-    t = P.partOf x := by
-  have hx : x ∈ s := by
-    rw [← P.sUnion_eq]
-    exact mem_sUnion_of_mem hxt ht
-  obtain ⟨t', ⟨-, h⟩⟩ := P.exists_unique_of_mem_set hx
-  rw [h t ⟨ht, hxt⟩, h (P.partOf x) ⟨P.partOf_mem hx, P.mem_partOf hx⟩]
-
-/-- Noncomputably choose a representative from an equivalence class-/
-noncomputable def rep (P : Partition s) (ht : t ∈ P) : α := (P.nonempty_of_mem ht).some
-
-@[simp] lemma rep_mem (ht : t ∈ P) : P.rep ht ∈ t :=
-  (P.nonempty_of_mem ht).some_mem
-
-@[simp] lemma rep_mem' (ht : t ∈ P) : P.rep ht ∈ s :=
-  P.subset_of_mem ht <| rep_mem ht
-
-@[simp] lemma partOf_rep (ht : t ∈ P) : P.partOf (P.rep ht) = t :=
-  (eq_partOf_of_mem ht (P.rep_mem ht)).symm
-
-lemma finite_of_finite (P : Partition s) (hs : s.Finite) : (P : Set (Set α)).Finite :=
-  hs.finite_subsets.subset fun _ ↦ subset_of_mem
+@[simp]
+lemma subset_sUnion_iff_mem {S : Set (Set α)} (ht : t ∈ P) (hSP : S ⊆ P.parts) :
+    t ⊆ ⋃₀ S ↔ t ∈ S := by
+  rw [← subset_sUnion_and_mem_iff_mem hSP]
+  simp [ht]
 
 end Set
 
 section Rel
 
-variable {s t : Set α} {a b : α} {P : Partition s}
+variable {S T : Set α} {a b : α} {P : Partition (Set α)}
 
-lemma symm_iff_of {α : Type*} (r : α → α → Prop) [IsSymm α r] {x y : α} : r x y ↔ r y x :=
-  ⟨fun h ↦ symm_of r h, fun h ↦ symm_of r h⟩
+-- lemma eqv_class_comm {r : α → α → Prop} [IsSymm α r] (x : α) : {y | r x y} = {y | r y x} := by
+--   simp_rw [comm]
 
-lemma refl_of_rel {α : Type*} (r : α → α → Prop) [IsSymm α r] [IsTrans α r] {x y : α}
-    (h : r x y) : r x x :=
-  trans_of r h (symm_of r h)
+-- lemma rel_iff_eqv_class_eq_right (hy : r y y) : r x y ↔ {z | r x z} = {z | r y z} := by
+--   simp_rw [Set.ext_iff, mem_setOf]
+--   exact ⟨fun hxy z ↦ ⟨fun hxz ↦ trans_of r (symm_of r hxy) hxz,
+--     fun hyz ↦ trans_of r hxy hyz⟩, fun h ↦ by rwa [h]⟩
 
-/-- A transitive, symmetric Binary relation `r` induces a partition of the set of elements on
-  which it is reflexive. -/
-@[simps] def ofRel (r : α → α → Prop) [IsTrans α r] [IsSymm α r] : Partition {x | r x x} where
-  parts := ((fun a ↦ {x | r a x}) '' {x | r x x})
-  indep := by
-    apply PairwiseDisjoint.sSupIndep
-    rintro _ ⟨i, -, rfl⟩ _ ⟨j, -,rfl⟩ hij
-    refine disjoint_iff_forall_ne.2 ?_
-    rintro a (ha : r _ _) _ (hb : r _ _) rfl
-    simp only [ne_eq, Set.ext_iff, mem_setOf_eq, not_forall] at hij
-    obtain ⟨y, hy⟩ := hij
-    exact hy ⟨fun hiy ↦ trans_of r hb (trans_of r (symm_of r ha) hiy),
-      fun hjy ↦ trans_of r ha (trans_of r (symm_of r hb) hjy)⟩
-  bot_notMem := by
-    simp only [bot_eq_empty, mem_image, mem_setOf_eq, eq_empty_iff_forall_notMem, not_exists,
-      not_and, not_forall, not_not]
-    exact fun x hx ↦ ⟨x,hx⟩
-  sSup_eq' := by
-    rw [sSup_eq_sUnion, subset_antisymm_iff]
-    simp only [sUnion_image, mem_setOf_eq, iUnion_subset_iff, setOf_subset_setOf]
-    refine ⟨fun i _ a ha ↦ trans_of r (symm_of r ha) ha, fun i (hi : r i i) ↦ ?_⟩
-    simp only [mem_iUnion, mem_setOf_eq, exists_prop]
-    exact ⟨i, hi, hi⟩
+-- lemma rel_iff_eqv_class_eq_left (hx : r x x) : r x y ↔ {z | r x z} = {z | r y z} := by
+--   rw [comm_of r, rel_iff_eqv_class_eq_right hx, eq_comm]
 
-/-- A version of `Partition.ofRel` with alternative definitional properties. -/
-@[simps!] def ofRel' (r : α → α → Prop) [IsTrans α r] [IsSymm α r] (hs : s = {x | r x x}) :=
-  (ofRel r).congr hs.symm
+-- lemma eqv_class_mem_ofRel (h : r x x) : {y | r x y} ∈ ofRel r :=
+--   ⟨x, h, rfl⟩
 
-variable {r : α → α → Prop} [IsSymm α r] [IsTrans α r] {s : Set α}
+-- @[simp] lemma mem_ofRel_iff {t : Set α} :
+--     t ∈ ofRel r ↔ ∃ x, r x x ∧ t = {y | r x y} := by
+--   simp_rw [eq_comm (a := t)]; rfl
 
-lemma eqv_class_comm {r : α → α → Prop} [IsSymm α r] (x : α) : {y | r x y} = {y | r y x} := by
-  simp_rw [symm_iff_of]
+-- @[simp] lemma mem_ofRel'_iff {t : Set α} (hs : s = {x | r x x}):
+--     t ∈ ofRel' r hs ↔ ∃ x ∈ s, t = {y | r x y} := by
+--   subst hs
+--   simp [ofRel', mem_congr_iff, mem_ofRel_iff]
 
-lemma rel_iff_eqv_class_eq_right (hy : r y y) : r x y ↔ {z | r x z} = {z | r y z} := by
-  simp_rw [Set.ext_iff, mem_setOf]
-  exact ⟨fun hxy z ↦ ⟨fun hxz ↦ trans_of r (symm_of r hxy) hxz,
-    fun hyz ↦ trans_of r hxy hyz⟩, fun h ↦ by rwa [h]⟩
-
-lemma rel_iff_eqv_class_eq_left (hx : r x x) : r x y ↔ {z | r x z} = {z | r y z} := by
-  rw [symm_iff_of r, rel_iff_eqv_class_eq_right hx, eq_comm]
-
-lemma eqv_class_mem_ofRel (h : r x x) : {y | r x y} ∈ ofRel r :=
-  ⟨x, h, rfl⟩
-
-@[simp] lemma mem_ofRel_iff {t : Set α} :
-    t ∈ ofRel r ↔ ∃ x, r x x ∧ t = {y | r x y} := by
-  simp_rw [eq_comm (a := t)]; rfl
-
-@[simp] lemma mem_ofRel'_iff {t : Set α} (hs : s = {x | r x x}):
-    t ∈ ofRel' r hs ↔ ∃ x ∈ s, t = {y | r x y} := by
-  subst hs
-  simp [ofRel', mem_congr_iff, mem_ofRel_iff]
-
-lemma class_nonempty {t : Set α} (ht : t ∈ ofRel r) : t.Nonempty := by
-  obtain ⟨x, hx, rfl⟩ := ht; exact ⟨x, hx⟩
+-- lemma class_nonempty {t : Set α} (ht : t ∈ ofRel r) : t.Nonempty :=
+--   nonempty_of_mem_fibers ht
 
 /-- Every partition of `s : Set α` induces a transitive, symmetric Binary relation on `α`
   whose equivalence classes are the parts of `P`. The relation is irreflexive outside `s`.  -/
-def Rel (P : Partition s) (a b : α) : Prop :=
+def Rel (P : Partition (Set α)) (a b : α) : Prop :=
   ∃ t ∈ P, a ∈ t ∧ b ∈ t
 
 lemma Rel.exists (h : P.Rel x y) : ∃ t ∈ P, x ∈ t ∧ y ∈ t :=
   h
 
-lemma Rel.forall (h : P.Rel x y) (ht : t ∈ P) : x ∈ t ↔ y ∈ t := by
-  obtain ⟨t', ht', hx, hy⟩ := h
+lemma Rel.forall (h : P.Rel x y) (ht : T ∈ P) : x ∈ T ↔ y ∈ T := by
+  obtain ⟨t, ht', hx, hy⟩ := h
   exact ⟨fun h ↦ by rwa [P.eq_of_mem_of_mem ht ht' h hx],
     fun h ↦ by rwa [P.eq_of_mem_of_mem ht ht' h hy]⟩
 
-lemma rel_of_mem_of_mem (ht : t ∈ P) (ha : a ∈ t) (hb : b ∈ t) : P.Rel a b :=
-  ⟨t, ht, ha, hb⟩
+lemma rel_of_mem_of_mem (ht : T ∈ P) (ha : a ∈ T) (hb : b ∈ T) : P.Rel a b :=
+  ⟨T, ht, ha, hb⟩
 
-lemma rel_self_of_mem (ht : t ∈ P) (hx : x ∈ t) : P.Rel x x :=
+lemma rel_self_of_mem (ht : T ∈ P) (hx : x ∈ T) : P.Rel x x :=
   rel_of_mem_of_mem ht hx hx
 
-instance (P : Partition s) : IsSymm α P.Rel where
-  symm _ _ := fun ⟨t, ht, ha, hb⟩ ↦ ⟨t, ht, hb, ha⟩
+lemma rel_self_of_mem_supp (hx : x ∈ P.supp) : P.Rel x x := by
+  obtain ⟨t, ht, hxt⟩ := mem_supp_iff.mp hx
+  exact rel_self_of_mem ht hxt
 
-instance (P : Partition s) : IsTrans α P.Rel where
-  trans a b c := fun ⟨t, htP, ha, hb⟩ ⟨t', ht'P, hb', hc'⟩ ↦
-    ⟨t, htP, ha, by rwa [eq_of_mem_of_mem htP ht'P hb hb']⟩
+lemma rel_symmectric (P : Partition (Set α)) : Symmetric (P.Rel) :=
+  fun _ _ ⟨t, ht, ha, hb⟩ ↦ ⟨t, ht, hb, ha⟩
 
-lemma Rel.symm {P : Partition s} (h : P.Rel x y) : P.Rel y x :=
+instance (P : Partition (Set α)) : IsSymm α P.Rel where
+  symm := P.rel_symmectric
+
+lemma rel_transitive (P : Partition (Set α)) : Transitive (P.Rel) := by
+  intro _ _ _ ⟨t, ht, ha, hb⟩ ⟨t', ht', hb', hc⟩
+  exact ⟨t, ht, ha, by rwa [eq_of_mem_of_mem ht ht' hb hb']⟩
+
+instance (P : Partition (Set α)) : IsTrans α P.Rel where
+  trans := P.rel_transitive
+
+lemma Rel.symm {P : Partition (Set α)} (h : P.Rel x y) : P.Rel y x :=
   symm_of P.Rel h
 
-lemma rel_comm {P : Partition s} : P.Rel x y ↔ P.Rel y x :=
+lemma rel_comm {P : Partition (Set α)} : P.Rel x y ↔ P.Rel y x :=
   ⟨Rel.symm, Rel.symm⟩
 
-lemma Rel.trans {P : Partition s} (hxy : P.Rel x y) (hyz : P.Rel y z) : P.Rel x z :=
+lemma Rel.trans {P : Partition (Set α)} (hxy : P.Rel x y) (hyz : P.Rel y z) : P.Rel x z :=
   trans_of P.Rel hxy hyz
 
-lemma Rel.mem_left {P : Partition s} (h : P.Rel x y) : x ∈ s := by
+lemma Rel.mem_left {P : Partition (Set α)} (h : P.Rel x y) : x ∈ P.supp := by
   obtain ⟨t, htP, hxt, -⟩ := h
   exact subset_of_mem htP hxt
 
-lemma Rel.mem_right {P : Partition s} (h : P.Rel x y) : y ∈ s :=
+lemma Rel.mem_right {P : Partition (Set α)} (h : P.Rel x y) : y ∈ P.supp :=
   h.symm.mem_left
 
 lemma rel_iff_exists : P.Rel x y ↔ ∃ t ∈ P, x ∈ t ∧ y ∈ t := Iff.rfl
 
-lemma rel_iff_partOf_eq_partOf (P : Partition s) (hx : x ∈ s) (hy : y ∈ s) :
+@[simp]
+lemma domain_rel {P : Partition (Set α)} : domain P.Rel = P.supp := by
+  ext x
+  simp only [mem_domain_iff, Rel, mem_supp_iff]
+  exact ⟨fun ⟨y, S, hS, hxS, _⟩ => ⟨S, hS, hxS⟩, fun ⟨S, hS, hxS⟩ => ⟨x, S, hS, hxS, hxS⟩⟩
+
+@[simp]
+lemma codomain_rel {P : Partition (Set α)} : codomain P.Rel = P.supp := by
+  rw [← domain_eq_codomain, domain_rel]
+
+lemma le_of_rel_le {P Q : Partition (Set α)} (h : P.Rel ≤ Q.Rel) : P ≤ Q := by
+  intro S hS
+  obtain ⟨x, hxS⟩ := nonempty_of_mem hS
+  obtain ⟨T, hT, hxT, -⟩ := h x x (rel_self_of_mem hS hxS)
+  use T, hT
+  rintro a haS
+  obtain ⟨T', hT', haT', hxT'⟩ := h a x ⟨S, hS, haS, hxS⟩
+  obtain rfl := eq_of_mem_of_mem hT hT' hxT hxT'
+  exact haT'
+
+lemma rel_le_of_le {P Q : Partition (Set α)} (h : P ≤ Q) : P.Rel ≤ Q.Rel := by
+  intro x y ⟨S, hS, hxS, hyS⟩
+  obtain ⟨T, hT, hST⟩ := h S hS
+  exact ⟨T, hT, hST hxS, hST hyS⟩
+
+lemma rel_le_iff_le {P Q : Partition (Set α)} : P.Rel ≤ Q.Rel ↔ P ≤ Q :=
+  ⟨le_of_rel_le, rel_le_of_le⟩
+
+lemma rel_inj {P Q : Partition (Set α)} (h : P.Rel = Q.Rel) : P = Q :=
+  le_antisymm (le_of_rel_le h.le) (le_of_rel_le h.ge)
+
+lemma rel_inj_iff {P Q : Partition (Set α)} : P.Rel = Q.Rel ↔ P = Q :=
+  ⟨fun h => rel_inj h, fun h => h ▸ rfl⟩
+
+/-- A transitive, symmetric Binary relation `r` induces a partition of the set of elements on
+  which it is reflexive. -/
+@[simps] def ofRel (r : α → α → Prop) [IsTrans α r] [IsSymm α r] : Partition (Set α) where
+  parts := fibers r
+  indep := PairwiseDisjoint.sSupIndep fibers_pairwiseDisjoint
+  bot_notMem := emptySet_notMem_fibers r
+
+@[simp]
+lemma ofRel_supp {r : α → α → Prop} [IsSymm α r] [IsTrans α r] : (ofRel r).supp = domain r :=
+  sUnion_fibers r
+
+lemma rel_ofRel_eq {r : α → α → Prop} [IsTrans α r] [IsSymm α r] : (ofRel r).Rel = r := by
+  ext a b
+  exact ⟨fun ⟨S, ⟨c, ⟨d, hdc⟩, heq⟩, haS, hbS⟩ => trans' (heq ▸ haS) (symm (heq ▸ hbS)),
+    fun hab => ⟨fiber r b, fiber_mem_fibers hab, hab, refl_of_right hab⟩⟩
+
+lemma ofRel_rel_eq (P : Partition (Set α)) : ofRel P.Rel = P := by
+  apply rel_inj
+  rw [rel_ofRel_eq]
+
+lemma fibers_rel_eq : fibers P.Rel = P.parts := by
+  rw [Set.ext_iff]
+  exact (ofRel P.Rel).ext_iff.mp <| ofRel_rel_eq P
+
+instance {S : Set (Partition (Set α))} : IsSymm α (sSup <| Partition.Rel '' S) where
+  symm := sSup_symmtric (fun _ ⟨_, _, heq⟩ => heq ▸ inferInstance)
+
+instance {S : Set (Partition (Set α))} : IsSymm α (sInf <| Partition.Rel '' S) where
+  symm := sInf_symmtric (fun _ ⟨_, _, heq⟩ => heq ▸ inferInstance)
+
+instance {S : Set (Partition (Set α))} : IsTrans α (sInf <| Partition.Rel '' S) where
+  trans := sInf_transitive (fun _ ⟨_, _, heq⟩ => heq ▸ inferInstance)
+
+instance : CompleteLattice (Partition (Set α)) where
+  sup P Q := ofRel <| TransClosure (P.Rel ⊔ Q.Rel)
+  le_sup_left P Q := by
+    rw [← rel_le_iff_le, rel_ofRel_eq]
+    exact le_trans le_sup_left (TransClosure.le_closure _)
+  le_sup_right P Q := by
+    rw [← rel_le_iff_le, rel_ofRel_eq]
+    exact le_trans le_sup_right (TransClosure.le_closure _)
+  sup_le r s t hrt hst := by
+    rw [← rel_le_iff_le] at hrt hst
+    rw [← rel_le_iff_le, rel_ofRel_eq]
+    exact ClosureOperator.closure_min (sup_le hrt hst) t.rel_transitive
+  inf P Q := ofRel <| P.Rel ⊓ Q.Rel
+  inf_le_left P Q := by
+    rw [← rel_le_iff_le, rel_ofRel_eq]
+    exact inf_le_left
+  inf_le_right P Q := by
+    rw [← rel_le_iff_le, rel_ofRel_eq]
+    exact inf_le_right
+  le_inf P Q R hPQR hPQR' := by
+    rw [← rel_le_iff_le] at hPQR hPQR'
+    rw [← rel_le_iff_le, rel_ofRel_eq]
+    exact le_inf hPQR hPQR'
+  sSup s := ofRel (TransClosure (sSup <| Partition.Rel '' s))
+  le_sSup S P hPS := by
+    rw [← rel_le_iff_le, rel_ofRel_eq]
+    exact le_trans (le_sSup <| mem_image_of_mem Partition.Rel hPS) (TransClosure.le_closure _)
+  sSup_le S r hrS := by
+    rw [← rel_le_iff_le, rel_ofRel_eq]
+    refine TransClosure.closure_min (sSup_le ?_) r.rel_transitive
+    rintro s ⟨s', hs', rfl⟩
+    exact rel_le_iff_le.mpr (hrS s' hs')
+  sInf S := ofRel (sInf <| Partition.Rel '' S)
+  le_sInf S r hrS := by
+    rw [← rel_le_iff_le, rel_ofRel_eq]
+    refine le_sInf <| ?_
+    rintro s ⟨s', hs', rfl⟩
+    exact rel_le_iff_le.mpr <| hrS s' hs'
+  sInf_le S r hrS := by
+    rw [← rel_le_iff_le, rel_ofRel_eq]
+    exact sInf_le <| mem_image_of_mem Partition.Rel hrS
+  le_top r := by simp
+  bot_le r := by simp
+
+end Rel
+
+section point
+
+variable {S T : Set α} {a b : α} {P : Partition (Set α)}
+
+/-- The part containing a given element of the set being partitioned. If `x ∉ s`, then `∅`.  -/
+def partOf (P : Partition (Set α)) (x : α) : Set α :=
+  fiber P.Rel x
+
+lemma exists_partOf_iff_mem : S ∈ P ↔ ∃ x ∈ P.supp, partOf P x = S := by
+  rw [← SetLike.mem_coe, ← mem_parts, ← fibers_rel_eq, mem_fibers_iff, codomain_rel]
+  rfl
+
+lemma partOf_mem (hx : x ∈ P.supp) : P.partOf x ∈ P := by
+  rw [exists_partOf_iff_mem]
+  use x
+
+lemma partOf_eq_empty (P : Partition (Set α)) (hx : x ∉ P.supp) : P.partOf x = ∅ :=
+  fiber_empty.mpr (by simpa)
+
+lemma mem_partOf (hx : x ∈ P.supp) : x ∈ P.partOf x :=
+  (mem_fiber_iff _).mpr <| rel_self_of_mem_supp hx
+
+lemma eq_partOf_of_mem (ht : T ∈ P) (hxt : x ∈ T) : T = P.partOf x := by
+  obtain ⟨y, hy, rfl⟩ := exists_partOf_iff_mem.mp ht
+  exact fiber_eq_of_mem (by exact hxt) <| rel_of_mem_of_mem ht hxt hxt
+
+/-- Noncomputably choose a representative from an equivalence class-/
+noncomputable def rep (P : Partition (Set α)) (ht : T ∈ P) : α := (P.nonempty_of_mem ht).some
+
+@[simp] lemma rep_mem (ht : T ∈ P) : P.rep ht ∈ T :=
+  (P.nonempty_of_mem ht).some_mem
+
+@[simp] lemma rep_mem' (ht : T ∈ P) : P.rep ht ∈ P.supp :=
+  P.subset_of_mem ht <| rep_mem ht
+
+@[simp] lemma partOf_rep (ht : T ∈ P) : P.partOf (P.rep ht) = T :=
+  (eq_partOf_of_mem ht (P.rep_mem ht)).symm
+
+lemma finite_of_finite (P : Partition (Set α)) (hs : P.supp.Finite) : (P : Set (Set α)).Finite :=
+  hs.finite_subsets.subset fun _ ↦ subset_of_mem
+
+lemma rel_iff_partOf_eq_partOf (P : Partition (Set α)) (hx : x ∈ P.supp) (hy : y ∈ P.supp) :
     P.Rel x y ↔ P.partOf x = P.partOf y := by
   refine ⟨fun ⟨t, htP, hxt, hyt⟩ ↦ ?_, fun h ↦ ⟨P.partOf x, P.partOf_mem hx, P.mem_partOf hx, ?_⟩⟩
   · rw [eq_partOf_of_mem (P.partOf_mem hx)]
     rwa [← eq_partOf_of_mem htP hxt]
   rw [h]
-  exact mem_partOf P hy
+  exact mem_partOf hy
 
-lemma rel_iff_partOf_eq_partOf' (P : Partition s) :
-    P.Rel x y ↔ ∃ (_ : x ∈ s) (_ : y ∈ s), P.partOf x = P.partOf y :=
+lemma rel_iff_partOf_eq_partOf' (P : Partition (Set α)) :
+    P.Rel x y ↔ ∃ (_ : x ∈ P.supp) (_ : y ∈ P.supp), P.partOf x = P.partOf y :=
   ⟨fun h ↦ ⟨h.mem_left, h.mem_right, (P.rel_iff_partOf_eq_partOf h.mem_left h.mem_right).1 h⟩,
     fun ⟨hx,hy,h⟩ ↦ (P.rel_iff_partOf_eq_partOf hx hy).2 h⟩
 
-lemma rel_iff_forall {P : Partition s} : P.Rel x y ↔ x ∈ s ∧ ∀ t ∈ P, x ∈ t ↔ y ∈ t := by
+lemma rel_iff_forall {P : Partition (Set α)} : P.Rel x y ↔ x ∈ P.supp ∧ ∀ t ∈ P, x ∈ t ↔ y ∈ t := by
   refine ⟨fun h ↦ ⟨h.mem_left, fun _ ↦ h.forall⟩,
     fun ⟨hxs, h⟩ ↦ ⟨P.partOf x, P.partOf_mem hxs, P.mem_partOf hxs, ?_⟩⟩
   rw [← h _ (P.partOf_mem hxs)]
   exact P.mem_partOf hxs
 
-lemma setOf_rel_self_eq (P : Partition s) : {x | P.Rel x x} = s := by
+lemma setOf_rel_self_eq (P : Partition (Set α)) : {x | P.Rel x x} = P.supp := by
   refine subset_antisymm (fun x hx ↦ ?_) (fun x hx ↦ ?_)
   · obtain ⟨t, ht, hxP, -⟩ := hx
     exact subset_of_mem ht hxP
-  obtain ⟨t, ⟨ht, hxt⟩, -⟩ := P.exists_unique_of_mem_set hx
+  obtain ⟨t, ⟨ht, hxt⟩, -⟩ := P.exists_unique_of_mem_supp hx
   exact ⟨t, ht, hxt, hxt⟩
 
-lemma rel_self_iff_mem {P : Partition s} : P.Rel x x ↔ x ∈ s := by
+lemma rel_self_iff_mem {P : Partition (Set α)} : P.Rel x x ↔ x ∈ P.supp := by
   simp [← P.setOf_rel_self_eq]
 
-lemma setOf_rel_eq (ht : t ∈ P) (hx : x ∈ t) : {y | P.Rel x y} = t :=
+lemma setOf_rel_eq (ht : T ∈ P) (hx : x ∈ T) : {y | P.Rel x y} = T :=
   Set.ext fun y ↦ ⟨fun ⟨t', ht', hx', hy'⟩ ↦ by rwa [P.eq_of_mem_of_mem ht ht' hx hx'],
-    fun h ↦ ⟨t, ht, hx, h⟩⟩
+    fun h ↦ ⟨T, ht, hx, h⟩⟩
 
-lemma rep_rel (ht : t ∈ P) (hx : x ∈ t) : P.Rel x (P.rep ht) :=
-  ⟨t, ht, hx, P.rep_mem ht⟩
+lemma rep_rel (ht : T ∈ P) (hx : x ∈ T) : P.Rel x (P.rep ht) :=
+  ⟨T, ht, hx, P.rep_mem ht⟩
 
-@[simp] lemma rep_rel_self {P : Partition s} (ht : t ∈ P) : P.Rel (P.rep ht) (P.rep ht) :=
+@[simp] lemma rep_rel_self {P : Partition (Set α)} (ht : T ∈ P) : P.Rel (P.rep ht) (P.rep ht) :=
   rep_rel _ (P.rep_mem ht)
 
-lemma setOf_rel_rep_eq (ht : t ∈ P) : {x | P.Rel (P.rep ht) x} = t :=
+lemma setOf_rel_rep_eq (ht : T ∈ P) : {x | P.Rel (P.rep ht) x} = T :=
   setOf_rel_eq ht (P.rep_mem ht)
 
 /-- The `partOf x` is the set of `y` related to `x`. True even if `x ∉ s`, since both are `∅`.-/
-lemma setOf_rel_eq_partOf (P : Partition s) (x : α) : {y | P.Rel x y} = P.partOf x := by
-  by_cases hx : x ∈ s
+lemma setOf_rel_eq_partOf (P : Partition (Set α)) (x : α) : {y | P.Rel x y} = P.partOf x := by
+  by_cases hx : x ∈ P.supp
   · rw [setOf_rel_eq (P.partOf_mem hx) (P.mem_partOf hx)]
   rw [partOf_eq_empty _ hx, eq_empty_iff_forall_notMem]
   exact fun y hxy ↦ hx <| Rel.mem_left hxy
 
-lemma setOf_rel_mem (P : Partition s) (hx : x ∈ s) : {y | P.Rel x y} ∈ P := by
-  obtain ⟨t, ⟨ht,hp⟩, -⟩ := P.exists_unique_of_mem_set hx
+lemma setOf_rel_mem (P : Partition (Set α)) (hx : x ∈ P.supp) : {y | P.Rel x y} ∈ P := by
+  obtain ⟨t, ⟨ht,hp⟩, -⟩ := P.exists_unique_of_mem_supp hx
   rwa [setOf_rel_eq ht hp]
 
-@[simp] lemma rel_congr (P : Partition s) (hst : s = t) : (P.congr hst).Rel = P.Rel := rfl
-
-lemma ofRel_rel_eq (P : Partition s) : ofRel' P.Rel P.setOf_rel_self_eq.symm = P := by
-  ext a
-  simp only [mem_ofRel'_iff]
-  refine ⟨?_, fun h ↦ ?_⟩
-  · rintro ⟨x,hx, rfl⟩
-    exact setOf_rel_mem _ hx
-  obtain ⟨x, hx⟩ := P.nonempty_of_mem h
-  exact ⟨x, (P.subset_of_mem h) hx, by rwa [setOf_rel_eq _ hx]⟩
-
-@[simp] lemma rel_ofRel_eq (r : α → α → Prop) [IsTrans α r] [IsSymm α r] : (ofRel r).Rel = r := by
-  ext a b
-  simp only [Rel, mem_ofRel_iff]
-  refine ⟨?_, fun h ↦ ⟨_, ⟨a, refl_of_rel r h, rfl⟩, refl_of_rel r h, h⟩⟩
-  rintro ⟨_, ⟨x, -, rfl⟩, ha, hb⟩
-  exact trans_of r (symm_of r ha) hb
-
-@[ext] theorem eq_of_rel_iff_rel {P P' : Partition s} (h : ∀ x y, P.Rel x y ↔ P'.Rel x y) :
+@[ext] theorem eq_of_rel_iff_rel {P P' : Partition (Set α)} (h : ∀ x y, P.Rel x y ↔ P'.Rel x y) :
     P = P' := by
   rw [← ofRel_rel_eq P, ← ofRel_rel_eq P']; congr; ext; exact h _ _
 
-@[simp] lemma discrete.rel_iff_eq : (Partition.discrete s).Rel a b ↔ a = b ∧ a ∈ s := by
-  simp only [Partition.discrete, le_eq_subset, Set.isAtom_iff]
+@[simp] lemma discrete.rel_iff_eq : (Partition.discrete S).Rel a b ↔ a = b ∧ a ∈ S := by
+  simp only [Partition.discrete, isAtom_iff, le_eq_subset]
   refine ⟨fun ⟨_, ⟨⟨x, rfl⟩, hxs⟩, hax, hbx⟩ ↦ by simp_all, ?_⟩
   rintro ⟨rfl, has⟩
-  exact (rel_iff_partOf_eq_partOf _ has has).mpr rfl
+  rw [rel_self_iff_mem]
+  exact ⟨{a}, ⟨⟨a, rfl⟩, singleton_subset_iff.mpr has⟩, rfl⟩
 
-lemma discrete.rel_iff_eq_of_mem (ha : a ∈ s) : (Partition.discrete s).Rel a b ↔ a = b := by
+lemma discrete.rel_iff_eq_of_mem (ha : a ∈ P.supp) :
+    (Partition.discrete P.supp).Rel a b ↔ a = b := by
   rw [discrete.rel_iff_eq, and_iff_left ha]
 
--- noncomputable instance : CompleteLattice (Partition s) where
---   sup P Q := ofRel' (Relation.TransGen <| P.Rel ⊔ Q.Rel) sorry
---   inf P Q := ofRel' (P.Rel ⊓ Q.Rel) sorry
---   sSup A := ofRel' (Relation.TransGen <| sSup <| (·.Rel) '' A) sorry
---   sInf A := ofRel' (sInf <| (·.Rel) '' A) sorry
-
-end Rel
+end point
 
 section RepFun
 
-variable {a b : α} {s : Set α} {P : Partition s}
+variable {a b : α} {s : Set α} {P : Partition (Set α)}
 
-structure RepFun (P : Partition s) where
+structure RepFun (P : Partition (Set α)) where
   (toFun : α → α)
-  (apply_eq_self_of_notMem : ∀ a ∉ s, toFun a = a)
-  (rel_apply_of_mem : ∀ a ∈ s, P.Rel a (toFun a))
+  (apply_eq_self_of_notMem : ∀ a ∉ P.supp, toFun a = a)
+  (rel_apply_of_mem : ∀ a ∈ P.supp, P.Rel a (toFun a))
   (apply_eq_of_rel : ∀ a b, P.Rel a b → toFun a = toFun b)
 
 instance : FunLike (RepFun P) α α where
   coe := RepFun.toFun
   coe_injective' f f' := by cases f; cases f'; simp
 
-@[simp] lemma RepFun.mk_apply (P : Partition s) (f) (h₁ : ∀ a ∉ s, f a = a)
-  (h₂ : ∀ a ∈ s, P.Rel a (f a)) (h₃) (x : α) : (RepFun.mk f h₁ h₂ h₃) x = f x := rfl
+def RepFun.mk' (P : Partition (Set α)) (f : α → α) {p : α → Prop} (hP : ∀ {x}, x ∈ P.supp ↔ p x)
+    (h₁ : ∀ a, ¬ p a → f a = a) (h₂ : ∀ a, p a → P.Rel a (f a))
+    (h₃ : ∀ a b, P.Rel a b → f a = f b) : P.RepFun :=
+  ⟨f, fun a ha ↦ h₁ a (hP.not.mp ha), fun a ha ↦ h₂ a (hP.mp ha), h₃⟩
 
-lemma RepFun.apply_of_notMem (f : P.RepFun) (ha : a ∉ s) : f a = a :=
+@[simp] lemma RepFun.mk_apply (P : Partition (Set α)) (f) (h₁ : ∀ a ∉ P.supp, f a = a)
+  (h₂ : ∀ a ∈ P.supp, P.Rel a (f a)) (h₃) (x : α) : (RepFun.mk f h₁ h₂ h₃) x = f x := rfl
+
+lemma RepFun.apply_of_notMem (f : P.RepFun) (ha : a ∉ P.supp) : f a = a :=
   f.apply_eq_self_of_notMem a ha
 
-lemma RepFun.rel_apply (f : P.RepFun) (ha : a ∈ s) : P.Rel a (f a) :=
+lemma RepFun.rel_apply (f : P.RepFun) (ha : a ∈ P.supp) : P.Rel a (f a) :=
   f.rel_apply_of_mem a ha
 
-lemma RepFun.apply_mem (f : P.RepFun) (ha : a ∈ s) : f a ∈ s :=
+lemma RepFun.rel_apply' (f : P.RepFun) {p : α → Prop} (hP : ∀ {x}, x ∈ P.supp ↔ p x) (ha : p a) :
+    P.Rel a (f a) := f.rel_apply <| hP.mpr ha
+
+lemma RepFun.apply_mem (f : P.RepFun) (ha : a ∈ P.supp) : f a ∈ P.supp :=
   (f.rel_apply ha).mem_right
+
+lemma RepFun.apply_mem' (f : P.RepFun) {p : α → Prop} (hP : ∀ {x}, x ∈ P.supp ↔ p x) (ha : p a) :
+    p (f a) := hP.mp <| f.apply_mem <| hP.mpr ha
 
 lemma RepFun.apply_eq_apply (f : P.RepFun) (hab : P.Rel a b) : f a = f b :=
   f.apply_eq_of_rel a b hab
 
-lemma RepFun.rel_of_apply_eq_apply (f : P.RepFun) (ha : a ∈ s) (hab : f a = f b) : P.Rel a b := by
+lemma RepFun.rel_of_apply_eq_apply (f : P.RepFun) (ha : a ∈ P.supp) (hab : f a = f b) :
+    P.Rel a b := by
   refine (f.rel_apply ha).trans ?_
   rw [hab, P.rel_comm]
   refine f.rel_apply <| by_contra fun hb ↦ ?_
@@ -622,31 +764,31 @@ lemma RepFun.rel_of_apply_eq_apply (f : P.RepFun) (ha : a ∈ s) (hab : f a = f 
 
 lemma RepFun.rel_of_ne_of_apply_eq_apply (f : P.RepFun) (hne : a ≠ b) (hab : f a = f b) :
     P.Rel a b := by
-  obtain (ha | ha) := em (a ∈ s); exact f.rel_of_apply_eq_apply ha hab
-  obtain (hb | hb) := em (b ∈ s); exact (f.rel_of_apply_eq_apply hb hab.symm).symm
+  obtain (ha | ha) := em (a ∈ P.supp); exact f.rel_of_apply_eq_apply ha hab
+  obtain (hb | hb) := em (b ∈ P.supp); exact (f.rel_of_apply_eq_apply hb hab.symm).symm
   rw [f.apply_of_notMem ha, f.apply_of_notMem hb] at hab; contradiction
 
-lemma RepFun.apply_eq_apply_iff_rel (f : P.RepFun) (ha : a ∈ s) : f a = f b ↔ P.Rel a b :=
+lemma RepFun.apply_eq_apply_iff_rel (f : P.RepFun) (ha : a ∈ P.supp) : f a = f b ↔ P.Rel a b :=
   ⟨f.rel_of_apply_eq_apply ha, f.apply_eq_apply⟩
 
 lemma RepFun.apply_eq_apply_iff_rel_of_ne (f : P.RepFun) (hne : a ≠ b) : f a = f b ↔ P.Rel a b :=
   ⟨f.rel_of_ne_of_apply_eq_apply hne, f.apply_eq_apply⟩
 
 @[simp] lemma RepFun.idem (f : P.RepFun) (a : α) : f (f a) = f a := by
-  obtain (ha | ha) := em (a ∈ s)
+  obtain (ha | ha) := em (a ∈ P.supp)
   · rw [eq_comm, f.apply_eq_apply_iff_rel ha]
     exact f.rel_apply ha
   simp_rw [f.apply_of_notMem ha]
 
-lemma RepFun.image_subset_self (f : P.RepFun) : f '' s ⊆ s := by
+lemma RepFun.image_subset_self (f : P.RepFun) : f '' P.supp ⊆ P.supp := by
   rintro _ ⟨a,ha,rfl⟩; exact f.apply_mem ha
 
 /-- Any partially defined `RepFun` extends to a complete one. -/
-lemma exists_extend_partial_repFun (P : Partition s) {t : Set α} (f₀ : t → α)
-    (h_notMem : ∀ x : t, x.1 ∉ s → f₀ x = x) (h_mem : ∀ x : t, x.1 ∈ s → P.Rel x (f₀ x))
+lemma exists_extend_partial_repFun (P : Partition (Set α)) {t : Set α} (f₀ : t → α)
+    (h_notMem : ∀ x : t, x.1 ∉ P.supp → f₀ x = x) (h_mem : ∀ x : t, x.1 ∈ P.supp → P.Rel x (f₀ x))
     (h_eq : ∀ x y : t, P.Rel x y → f₀ x = f₀ y) : ∃ (f : P.RepFun), ∀ x : t, f x = f₀ x := by
   classical
-  set f : α → α := fun a ↦ if ha : a ∈ s then
+  set f : α → α := fun a ↦ if ha : a ∈ P.supp then
     (if hb : ∃ b : t, P.Rel a b then f₀ hb.choose else P.rep (P.partOf_mem ha)) else a with hf
   refine ⟨RepFun.mk f (fun a ha ↦ by simp [hf, ha]) (fun a ha ↦ ?_) (fun a b hab ↦ ?_), fun a ↦ ?_⟩
   · simp only [hf, ha, ↓reduceDIte]
@@ -662,7 +804,7 @@ lemma exists_extend_partial_repFun (P : Partition s) {t : Set α} (f₀ : t → 
     congr
     rwa [← rel_iff_partOf_eq_partOf _ hab.mem_left hab.mem_right]
   change f a = f₀ a
-  obtain (ha | ha) := em (a.1 ∈ s)
+  obtain (ha | ha) := em (a.1 ∈ P.supp)
   · simp only [hf, ha, ↓reduceDIte]
     split_ifs with h
     · exact Eq.symm <| h_eq _ _ h.choose_spec
@@ -671,17 +813,17 @@ lemma exists_extend_partial_repFun (P : Partition s) {t : Set α} (f₀ : t → 
 
 /-- For any set `t` containining no two distinct related elements, there is a `RepFun` equal to
 the identity on `t`. -/
-lemma exists_extend_partial_repFun' (P : Partition s) {t : Set α}
+lemma exists_extend_partial_repFun' (P : Partition (Set α)) {t : Set α}
     (h : ∀ ⦃x y⦄, x ∈ t → y ∈ t → P.Rel x y → x = y) : ∃ (f : P.RepFun), EqOn f id t := by
   simpa using P.exists_extend_partial_repFun (fun x : t ↦ x) (by simp)
     (by simp [P.rel_self_iff_mem]) (fun x y ↦ h x.2 y.2)
 
-lemma nonempty_repFun (P : Partition s) : Nonempty P.RepFun := by
+lemma nonempty_repFun (P : Partition (Set α)) : Nonempty P.RepFun := by
   obtain ⟨f, -⟩ := P.exists_extend_partial_repFun' (t := ∅) (by simp)
   exact ⟨f⟩
 
 @[simp] theorem repFun_repFun (f f' : P.RepFun) (x : α) : f (f' x) = f x := by
-  obtain (hx | hx) := em (x ∈ s)
+  obtain (hx | hx) := em (x ∈ P.supp)
   · exact f.apply_eq_apply (f'.rel_apply hx).symm
   rw [f'.apply_of_notMem hx, f.apply_of_notMem hx]
 
@@ -689,10 +831,10 @@ lemma nonempty_repFun (P : Partition s) : Nonempty P.RepFun := by
     (f : α → α) = id := by
   ext x
   obtain (hx | hx) := em (x ∈ s)
-  · have hx' := f.rel_apply hx
-    simp only [discrete.rel_iff_eq] at hx'
+  · have hx' := f.rel_apply (supp_discrete s ▸ hx)
+    rw [discrete.rel_iff_eq] at hx'
     exact hx'.1.symm
-  rw [f.apply_of_notMem hx, id]
+  rw [f.apply_of_notMem (supp_discrete s |>.symm ▸ hx), id]
 
 lemma RepFun.coeFun_eq_id_of_eq_discrete  (f : P.RepFun) (hP : P = Partition.discrete s) :
     (f : α → α) = id := by
@@ -709,17 +851,17 @@ lemma RepFun.coeFun_eq_id_of_eq_discrete  (f : P.RepFun) (hP : P = Partition.dis
 
 -- /-- If `a ∈ s`, noncomputably choose an element in the same cell of `P` as some `a : α`.
 -- If `a ∉ s`, is equal to `a`. -/
--- noncomputable def rep' (P : Partition s) (a : α) : α :=
+-- noncomputable def rep' (P : Partition (Set α)) (a : α) : α :=
 --     if h : a ∈ s then P.rep (P.partOf_mem h) else a
 
--- lemma rep'_eq_rep (P : Partition s) (ha : a ∈ s) : P.rep' a = P.rep (P.partOf_mem ha) := by
+-- lemma rep'_eq_rep (P : Partition (Set α)) (ha : a ∈ s) : P.rep' a = P.rep (P.partOf_mem ha) := by
 --   rw [rep', dif_pos ha]
 
--- lemma rel_rep' (P : Partition s) (ha : a ∈ s) : P.Rel a (P.rep' a) := by
+-- lemma rel_rep' (P : Partition (Set α)) (ha : a ∈ s) : P.Rel a (P.rep' a) := by
 --   rw [P.rep'_eq_rep ha]
 --   exact P.rep_rel (P.partOf_mem ha) (P.mem_partOf ha)
 
--- lemma rep'_eq_self_of_notMem (P : Partition s) (ha : a ∉ s) : P.rep' a = a := by
+-- lemma rep'_eq_self_of_notMem (P : Partition (Set α)) (ha : a ∉ s) : P.rep' a = a := by
 --   rw [rep', dif_neg ha]
 
 -- lemma rel_iff_rep'_eq_rep' (ha : a ∈ s) (hb : b ∈ s) : P.Rel a b ↔ P.rep' a = P.rep' b := by
@@ -733,21 +875,6 @@ lemma RepFun.coeFun_eq_id_of_eq_discrete  (f : P.RepFun) (hP : P = Partition.dis
 
 end RepFun
 
-
-end Partition
-section Fiber
-open Function
-
-instance {r : α → α → Prop} [IsRefl α r] {f : β → α} : IsRefl β (r on f) where
-  refl a := refl (f a)
-
-instance {r : α → α → Prop} [IsSymm α r] {f : β → α} : IsSymm β (r on f) where
-  symm a _ := symm (a := f a)
-
-instance {r : α → α → Prop} [IsTrans α r] {f : β → α} : IsTrans β (r on f) where
-  trans a _ _ := _root_.trans (a := f a)
-
-namespace Partition
 
 -- def Fiber (f : α → β) : Partition (univ : Set α) := Partition.ofRel' (Eq on f) <| by ext a; simp
 
